format-version: 1.2
date: 22:07:2020 11:31
saved-by: dwaring
auto-generated-by: convert_obo.pl/1.1
remark: This file was converted to an SGN-compatible obo file from a standard obo file [./oat.obo]
default-namespace: oat_trait
ontology: CO_350

[Typedef]
id: method_of
name: method_of
is_transitive: true

[Typedef]
id: scale_of
name: scale_of
is_transitive: true

[Typedef]
id: variable_of
name: variable_of

[Term]
id: CO_350:ROOT
name: Oat traits
namespace: oat_trait

[Term]
id: CO_350:Abiotic_stress
name: Abiotic stress trait
namespace: oat_trait
is_a: CO_350:ROOT

[Term]
id: CO_350:Quality
name: Quality trait
namespace: oat_trait
is_a: CO_350:ROOT

[Term]
id: CO_350:Biochemical
name: Biochemical trait
namespace: oat_trait
is_a: CO_350:ROOT

[Term]
id: CO_350:Phenological
name: Phenological trait
namespace: oat_trait
is_a: CO_350:ROOT

[Term]
id: CO_350:Physiological
name: Physiological traits
namespace: oat_trait
is_a: CO_350:ROOT

[Term]
id: CO_350:Metabolite
name: Metabolite trait
namespace: oat_trait
is_a: CO_350:ROOT

[Term]
id: CO_350:Morphological
name: Morphological trait
namespace: oat_trait
is_a: CO_350:ROOT

[Term]
id: CO_350:Biotic_stress
name: Biotic stress trait
namespace: oat_trait
is_a: CO_350:ROOT

[Term]
id: CO_350:Agronomic
name: Agronomic trait
namespace: oat_trait
is_a: CO_350:ROOT

[Term]
id: CO_350:0000081
name: Barley yellow dwarf virus incidence
namespace: oat_trait
def: "Percentage of plants in a plot showing symptoms of barley yellow dwarf virus." []
synonym: "BYDV incidence" EXACT []
is_a: CO_350:Biotic_stress

[Term]
id: CO_350:0000036
name: Beta-glucan content
namespace: oat_trait
def: "Amount of beta-glucan present in the groat expressed as a percentage of the entire groat." []
synonym: "BeGlCnt" EXACT []
is_a: CO_350:Biochemical

[Term]
id: CO_350:0000039
name: Broken groats
namespace: oat_trait
def: "The amount of broken groats after de-hulling, expressed as a percentage of the weight of the entire whole grain sample." []
synonym: "BrGrt" EXACT []
is_a: CO_350:Quality

[Term]
id: CO_350:0000042
name: Dietary fiber content
namespace: oat_trait
def: "Dietary fiber content" []
synonym: "DietFibCnt" EXACT []
is_a: CO_350:Biochemical

[Term]
id: CO_350:0000093
name: Fusarium head blight incidence
namespace: oat_trait
def: "Percentage of plants in a plot showing Fusarium head blight symptoms." []
synonym: "FHB incidence" EXACT []
is_a: CO_350:Biotic_stress

[Term]
id: CO_350:0000066
name: Grain plumpness
namespace: oat_trait
def: "The amount of a grain sample that does not pass through the holes of a sieve of defined size, expressed as a percentage weight of the entire sample." []
synonym: "GrPlum" EXACT []
is_a: CO_350:Morphological

[Term]
id: CO_350:0000048
name: Grain protein content
namespace: oat_trait
def: "The amount of protein in the grain, expressed as a percentage of the whole grain." []
synonym: "GrPtnCnt" EXACT []
is_a: CO_350:Biochemical

[Term]
id: CO_350:0000009
name: Groat content
namespace: oat_trait
def: "Groat content" []
synonym: "GrtCnt" EXACT []
is_a: CO_350:Agronomic

[Term]
id: CO_350:0000051
name: Groat oil content
namespace: oat_trait
def: "The amount of oil in the groat, expressed as a percentage of the groat." []
synonym: "GrtOilCnt" EXACT []
is_a: CO_350:Biochemical

[Term]
id: CO_350:0000054
name: Groat protein content
namespace: oat_trait
def: "The amount of protein in the groat, expressed as a percentage of the groat." []
synonym: "GrtPtnCnt" EXACT []
is_a: CO_350:Biochemical

[Term]
id: CO_350:0000015
name: Lodging incidence
namespace: oat_trait
def: "Measure of the percentage of the stems of plants in a plot that have been permanently bent, usually as a result of adverse weather." []
synonym: "Lodg" EXACT []
is_a: CO_350:Abiotic_stress

[Term]
id: CO_350:0000099
name: Powdery mildew incidence
namespace: oat_trait
def: "Percentage of plants in a plot showing symptoms of powdery mildew." []
synonym: "Pwinc" EXACT []
is_a: CO_350:Biotic_stress

[Term]
id: CO_350:0000102
name: Root rot incidence
namespace: oat_trait
def: "Percentage of plants in a plot showing symptoms of root rot." []
synonym: "RRInc" EXACT []
is_a: CO_350:Biotic_stress

[Term]
id: CO_350:0000105
name: Smut incidence
namespace: oat_trait
def: "Percentage of plants in a plot showing symptoms of smut." []
synonym: "SmutInc" EXACT []
is_a: CO_350:Biotic_stress

[Term]
id: CO_350:0000108
name: Stem rust incidence
namespace: oat_trait
def: "Percentage of plants in a plot showing symptoms of stem rust." []
synonym: "Srinc" EXACT []
is_a: CO_350:Biotic_stress

[Term]
id: CO_350:0000030
name: Winter survival
namespace: oat_trait
def: "Percentage of plants in a plot sown in fall that are still growing in spring." []
synonym: "WS" EXACT []
is_a: CO_350:Abiotic_stress

[Term]
id: CO_350:0000117
name: Lodging severity
namespace: oat_trait
def: "Severity of lodging symptoms observed in a plot: lodged plants do not stand erect." []
synonym: "LodgSev" EXACT []
is_a: CO_350:Abiotic_stress

[Term]
id: CO_350:0000084
name: Barley yellow dwarf virus severity
namespace: oat_trait
def: "Severity of barley yellow dwarf virus symptoms observed in a plot." []
synonym: "BYDV severity" EXACT []
is_a: CO_350:Biotic_stress

[Term]
id: CO_350:0000090
name: Crown rust severity
namespace: oat_trait
def: "Crown rust severity." []
synonym: "CrnRst" EXACT []
is_a: CO_350:Biotic_stress

[Term]
id: CO_350:0000096
name: Leaf blotch severity
namespace: oat_trait
def: "Severity of leaf blotch symptoms observed in a plot." []
synonym: "Lbsev" EXACT []
is_a: CO_350:Biotic_stress

[Term]
id: CO_350:0000003
name: Breakage incidence
namespace: oat_trait
def: "Proportion of the stems in a plot that are snapped/broken." []
synonym: "Break" EXACT []
is_a: CO_350:Abiotic_stress

[Term]
id: CO_350:0000072
name: Groat color
namespace: oat_trait
def: "Color of the de-hulled grain: the groat." []
synonym: "GrtCol" EXACT []
is_a: CO_350:Morphological

[Term]
id: CO_350:0000000
name: Agronomic score
namespace: oat_trait
def: "Rating of overall agronomical attributes and health of oat plants in a plot." []
synonym: "AgrSc" EXACT []
is_a: CO_350:Agronomic

[Term]
id: CO_350:0000114
name: Stem rust severity
namespace: oat_trait
def: "Stem rust severity." []
synonym: "StmRst" EXACT []
is_a: CO_350:Biotic_stress

[Term]
id: CO_350:0000024
name: Relative canopy development
namespace: oat_trait
def: "Relative canopy development, each genotype is rated against the earliest genotypes, when those genotypes have a completely closed canopy." []
synonym: "RelCan" EXACT []
is_a: CO_350:Phenological

[Term]
id: CO_350:0000027
name: Snapback
namespace: oat_trait
def: "Snapback, or recovery to a vertical position, of the plant after being held at a 45 degree angle." []
synonym: "Snap" EXACT []
is_a: CO_350:Abiotic_stress

[Term]
id: CO_350:0000021
name: Plant height
namespace: oat_trait
def: "Height of plant from ground to top of flag leaf ligule." []
synonym: "PlntHtLig" EXACT []
is_a: CO_350:Agronomic

[Term]
id: CO_350:0000012
name: Heading time
namespace: oat_trait
def: "The time when heading occurs." []
synonym: "HdDays" EXACT []
is_a: CO_350:Phenological

[Term]
id: CO_350:0000018
name: Maturity time
namespace: oat_trait
def: "The time when maturity occurs" []
synonym: "MatDays" EXACT []
is_a: CO_350:Phenological

[Term]
id: CO_350:0000087
name: Crown rust infection type
namespace: oat_trait
def: "A qualitative analysis of the type of crown rust symptoms that are exhibited." []
synonym: "CRItype" EXACT []
is_a: CO_350:Biotic_stress

[Term]
id: CO_350:0000111
name: Stem rust infection type
namespace: oat_trait
def: "A qualitative analysis of the type of stem rust symptoms that are exhibited." []
synonym: "Srinftype" EXACT []
is_a: CO_350:Biotic_stress

[Term]
id: CO_350:0000078
name: Thousand grain weight
namespace: oat_trait
def: "The thousand grain weight." []
synonym: "TGW" EXACT []
is_a: CO_350:Quality

[Term]
id: CO_350:0000063
name: Undehulled seed
namespace: oat_trait
def: "Amount of undehulled seed remaining after dehulling." []
synonym: "UndehulledS" EXACT []
is_a: CO_350:Quality

[Term]
id: CO_350:0000075
name: Test weight
namespace: oat_trait
def: "A measure of the density or weight per unit volume of a grain at a standardized moisture level." []
synonym: "TstW" EXACT []
is_a: CO_350:Morphological

[Term]
id: CO_350:0000006
name: Grain yield
namespace: oat_trait
def: "Total weight of grains harvested per unit area." []
synonym: "GrYie" EXACT []
is_a: CO_350:Agronomic

[Term]
id: CO_350:0000523
name: Downy mildew severity
namespace: oat_trait
def: "Downy mildew severity." []
synonym: "DnyMd" EXACT []
is_a: CO_350:Biotic_stress

[Term]
id: CO_350:0000120
name: Grain moisture content
namespace: oat_trait
def: "Moisture content of grain." []
synonym: "MoiCon" EXACT []
is_a: CO_350:Agronomic

[Term]
id: CO_350:0000572
name: Lipid content
namespace: oat_trait
def: "The lipid content of the grain." []
synonym: "LpCnt" EXACT []
is_a: CO_350:Quality

[Term]
id: CO_350:0000045
name: Deoxynivalenol concentration
namespace: oat_trait
def: "Amount of the mycotoxin deoxynivalenol found in the grain after an infection by Fusarium sp." []
synonym: "DON concentration" EXACT []
is_a: CO_350:Biochemical

[Term]
id: CO_350:0000033
name: Avenanthramide content
namespace: oat_trait
def: "Avenanthramide content" []
synonym: "AveCnt" EXACT []
is_a: CO_350:Biochemical

[Term]
id: CO_350:0000060
name: Tocopherol concentration
namespace: oat_trait
def: "Tocopherol concentration" []
synonym: "TocophCtn" EXACT []
is_a: CO_350:Biochemical

[Term]
id: CO_350:0000057
name: Tocotrienol concentration
namespace: oat_trait
def: "Tocotrienol concentration" []
synonym: "TocotrCtn" EXACT []
is_a: CO_350:Biochemical

[Term]
id: CO_350:0005401
name: Freeze damage severity
namespace: oat_trait
def: "Severity of the symptoms of freeze damage observed in a plot" []
synonym: "FDS" EXACT []
is_a: CO_350:Abiotic_stress

[Term]
id: CO_350:0005402
name: Storm damage severity
namespace: oat_trait
def: "Severity of the damage inflicted by stormy weather" []
synonym: "SDS" EXACT []
is_a: CO_350:Abiotic_stress

[Term]
id: CO_350:0005403
name: Winter stress severity
namespace: oat_trait
def: "Mid-winter rating of the severity of the symptoms of winter stress observed in a plot" []
synonym: "WSS" EXACT []
is_a: CO_350:Abiotic_stress

[Term]
id: CO_350:0005404
name: Emergence
namespace: oat_trait
def: "Percentage of plants in a plot that have emerged" []
synonym: "PE" EXACT []
is_a: CO_350:Agronomic

[Term]
id: CO_350:0005405
name: Forage rating
namespace: oat_trait
def: "Yield potential in spring" []
synonym: "FR" EXACT []
is_a: CO_350:Agronomic

[Term]
id: CO_350:0005406
name: Phenotype score
namespace: oat_trait
def: "Relative rating of visual appeal that takes in to account plant vigor, diseases, etc." []
synonym: "PS" EXACT []
is_a: CO_350:Agronomic

[Term]
id: CO_350:0005407
name: Silage yield
namespace: oat_trait
def: "Total weight of silage per unit area" []
synonym: "SY" EXACT []
is_a: CO_350:Agronomic

[Term]
id: CO_350:0005408
name: Bird damage severity
namespace: oat_trait
def: "Severity of the symptoms of bird damage observed in a plot" []
synonym: "BDS" EXACT []
is_a: CO_350:Biotic_stress

[Term]
id: CO_350:0005409
name: Cereal leaf beetle damage severity
namespace: oat_trait
def: "Severity of larval feeding damage caused by cereal leaf beetle (Oulema malanopus)." []
synonym: "CLBS" EXACT []
is_a: CO_350:Biotic_stress

[Term]
id: CO_350:0005410
name: Stagonospora severity
namespace: oat_trait
def: "Severity of Stagonospora avenae f. sp. avenaria symptoms. Stagonospora causes leaf blotch and black stem of oat." []
synonym: "SAS" EXACT []
is_a: CO_350:Biotic_stress

[Term]
id: CO_350:0005411
name: GC-MS
namespace: oat_trait
def: "Gas chromatography mass spectrometry" []
synonym: "GCMS" EXACT []
is_a: CO_350:Metabolite

[Term]
id: CO_350:0005412
name: LC-MS
namespace: oat_trait
def: "Liquid chromatography mass spectrometry" []
synonym: "LCMS" EXACT []
is_a: CO_350:Metabolite

[Term]
id: CO_350:0005413
name: Growth habit
namespace: oat_trait
def: "Growth habit rating ranging from very upright spring type to very prostrate winter type" []
synonym: "GH" EXACT []
is_a: CO_350:Morphological

[Term]
id: CO_350:0005414
name: Hull color
namespace: oat_trait
def: "Hull color" []
synonym: "HC" EXACT []
is_a: CO_350:Morphological

[Term]
id: CO_350:0005415
name: Kernels per spikelet
namespace: oat_trait
def: "Average number of kernels per spikelet" []
synonym: "KPS" EXACT []
is_a: CO_350:Morphological

[Term]
id: CO_350:0005416
name: Leaf biomass
namespace: oat_trait
def: "An estimation of the leaf biomass" []
synonym: "LBM" EXACT []
is_a: CO_350:Morphological

[Term]
id: CO_350:0005417
name: Panicle length
namespace: oat_trait
def: "Average panicle length " []
synonym: "PL" EXACT []
is_a: CO_350:Morphological

[Term]
id: CO_350:0005418
name: Spikelets per panicle
namespace: oat_trait
def: "Average number of spikelets per panicle" []
synonym: "SPP" EXACT []
is_a: CO_350:Morphological

[Term]
id: CO_350:0005419
name: Avenanthramide relative abundance
namespace: oat_trait
def: "Relative abundance of avenanthramide estimated by UPLC" []
synonym: "AveAbd" EXACT []
is_a: CO_350:Biochemical

[Term]
id: CO_350:0005420
name: Dehulling efficiency
namespace: oat_trait
def: "Efficiency of dehulling seed by a machine" []
synonym: "DHE" EXACT []
is_a: CO_350:Quality

[Term]
id: CO_350:0005421
name: 3-acetyl-deoxynivalenol concentration
namespace: oat_trait
def: "Amount of the mycotoxin 3-acetyl-deoxynivalenol found in the grain after an infection by Fusarium sp." []
synonym: "DON3-acetyl" EXACT []
is_a: CO_350:Biochemical

[Term]
id: CO_350:0005422
name: Fatty acid content
namespace: oat_trait
def: "Fatty acid content of the grain" []
synonym: "FAC" EXACT []
is_a: CO_350:Biochemical

[Term]
id: CO_350:0005423
name: Groat flour falling number
namespace: oat_trait
def: "Flour falling number is used as an indirect measurement of the alpha amylase content of the groat" []
synonym: "FFN" EXACT []
is_a: CO_350:Quality

[Term]
id: CO_350:0005424
name: Lutein content
namespace: oat_trait
def: "Lutein content" []
synonym: "LutCnt" EXACT []
is_a: CO_350:Quality

[Term]
id: CO_350:0005425
name: Phytoene content
namespace: oat_trait
def: "Phytoene content" []
synonym: "PhyeCnt" EXACT []
is_a: CO_350:Quality

[Term]
id: CO_350:0005426
name: Phytofluene content
namespace: oat_trait
def: "Phytofluene content" []
synonym: "PhyfCnt" EXACT []
is_a: CO_350:Quality

[Term]
id: CO_350:0005427
name: Seed quality
namespace: oat_trait
def: "Seed quality" []
synonym: "SQ" EXACT []
is_a: CO_350:Quality

[Term]
id: CO_350:0005428
name: Silage moisture content
namespace: oat_trait
def: "Moisture content of silage." []
synonym: "SMQ" EXACT []
is_a: CO_350:Quality

[Term]
id: CO_350:0005429
name: Total toco concentration
namespace: oat_trait
def: "Measure of the total -tocopherol and -tocotrienol content" []
synonym: "TocoCtn" EXACT []
is_a: CO_350:Quality

[Term]
id: CO_350:0005430
name: Tunaxanthin content
namespace: oat_trait
def: "Tunaxanthin content" []
synonym: "TaxCnt" EXACT []
is_a: CO_350:Quality

[Term]
id: CO_350:0005431
name: Violaxanthin content
namespace: oat_trait
def: "Violaxanthin content" []
synonym: "VaxCnt" EXACT []
is_a: CO_350:Quality

[Term]
id: CO_350:0005432
name: Zeaxanthin content
namespace: oat_trait
def: "Zeaxanthin content" []
synonym: "ZaxCnt" EXACT []
is_a: CO_350:Quality

[Term]
id: CO_350:0000082
name: Disease incidence observation
namespace: oat_trait_method
def: "Visual assessment of the percentage of plants in a plot showing symptoms of a specific disease." []
relationship: method_of CO_350:0000102
relationship: method_of CO_350:0000099
relationship: method_of CO_350:0000081
relationship: method_of CO_350:0000108
relationship: method_of CO_350:0000105

[Term]
id: CO_350:0000037
name: Beta-glucan content determination
namespace: oat_trait_method
def: "Measurement of beta glucan content on a dry weight basis using a lichenase enzymatic procedure." []
relationship: method_of CO_350:0000036

[Term]
id: CO_350:0000040
name: Broken groats determination
namespace: oat_trait_method
def: "Computation of the percentage of broken groats by weight after dehulling; calculated as the weight of broken groats divided by the total groat weight, multiplied by 100." []
relationship: method_of CO_350:0000039

[Term]
id: CO_350:0000043
name: Dietary fiber content determination
namespace: oat_trait_method
def: "Computation of total dietary fiber content  on a dry weight basis using wet chemistry." []
relationship: method_of CO_350:0000042

[Term]
id: CO_350:0000049
name: Grain protein content determination
namespace: oat_trait_method
def: "Computation of the percentage of protein in the whole grain as obtained using near-infrared spectroscopy (NIR)." []
relationship: method_of CO_350:0000048

[Term]
id: CO_350:0000010
name: Groat content determination (machine dehulled)
namespace: oat_trait_method
def: "Calculated as the weight of the groat divided by the weight of the whole grain, multiplied by 100. Kernels are typically dehulled using a Codema oat dehuller, which processes a 50 gram sample." []
relationship: method_of CO_350:0000009

[Term]
id: CO_350:0000052
name: Groat oil content determination
namespace: oat_trait_method
def: "Computation of the percentage of oil in the groat." []
relationship: method_of CO_350:0000051

[Term]
id: CO_350:0000055
name: Groat protein content determination
namespace: oat_trait_method
def: "Computation of the percentage of protein in the groat." []
relationship: method_of CO_350:0000054

[Term]
id: CO_350:0000016
name: Lodging incidence observation
namespace: oat_trait_method
def: "Visual assessement of the percentage of plants that lodged in a plot." []
relationship: method_of CO_350:0000015

[Term]
id: CO_350:0000031
name: Winter survival observation
namespace: oat_trait_method
def: "Visual assessement of the percentage of living plants in a plot." []
relationship: method_of CO_350:0000030

[Term]
id: CO_350:0000118
name: Lodging severity obervation
namespace: oat_trait_method
def: "Visual assessment of the severity of lodging observed in a plot." []
relationship: method_of CO_350:0000117

[Term]
id: CO_350:0000085
name: Disease severity observation
namespace: oat_trait_method
def: "Visual assessment of the severity of disease symptoms observed in a plot." []
relationship: method_of CO_350:0000096

[Term]
id: CO_350:0000004
name: Breakage incidence observation
namespace: oat_trait_method
def: "Rating based on the proportion of stems in a plot that are broken/snapped." []
relationship: method_of CO_350:0000003

[Term]
id: CO_350:0000073
name: Groat color observation
namespace: oat_trait_method
def: "Visual assessement of the color of the groat." []
relationship: method_of CO_350:0000072

[Term]
id: CO_350:0000001
name: Agronomic scoring
namespace: oat_trait_method
def: "Scored based on observance of factors limiting yield." []
relationship: method_of CO_350:0000000

[Term]
id: CO_350:0000025
name: Relative canopy development observation
namespace: oat_trait_method
def: "Visual assessment of the development of the canopy of a plot relative to genotypes with a closed canopy." []
relationship: method_of CO_350:0000024

[Term]
id: CO_350:0000028
name: Snapback rating
namespace: oat_trait_method
def: "Plants are held at a 45 degree angle and released. The snapback, or recovery to vertical position, is rated." []
relationship: method_of CO_350:0000027

[Term]
id: CO_350:0000022
name: Plant height measurement
namespace: oat_trait_method
def: "Measurement of the height of the whole plant from the soil surface to the tip of the panicle." []
relationship: method_of CO_350:0000021

[Term]
id: CO_350:0000079
name: TGW determination
namespace: oat_trait_method
def: "Measurement of the weight of 1000 well-developed whole grains." []
relationship: method_of CO_350:0000078

[Term]
id: CO_350:0000064
name: Undehulled seed determination
namespace: oat_trait_method
def: "Amount of undehulled seed remaining after passing a 50 gram sample through a Codema dehuller, under standard conditions, for 90 seconds." []
relationship: method_of CO_350:0000063

[Term]
id: CO_350:0000076
name: Test weight determination
namespace: oat_trait_method
def: "" []
relationship: method_of CO_350:0000075

[Term]
id: CO_350:0000007
name: Grain yield determination
namespace: oat_trait_method
def: "Measurement of the total weight of whole grains harvested per unit area." []
relationship: method_of CO_350:0000006

[Term]
id: CO_350:0000013
name: Heading date observation
namespace: oat_trait_method
def: "Record of the date on which heading occurs." []
relationship: method_of CO_350:0000012

[Term]
id: CO_350:0000019
name: Maturity date observation
namespace: oat_trait_method
def: "Record of the date on which maturity occurs." []
relationship: method_of CO_350:0000018

[Term]
id: CO_350:0000535
name: Oven determined grain moisture content computation
namespace: oat_trait_method
def: "Calculate the mositure content from fresh and dry grain weight." []
relationship: method_of CO_350:0000120

[Term]
id: CO_350:0000573
name: Lipid content measurement
namespace: oat_trait_method
def: "Measurement of the percentage of lipid content in grain; prediction obtained using near-infrared spectroscopy (NIR)." []
relationship: method_of CO_350:0000572

[Term]
id: CO_350:0000626
name: Stem rust severity - Estimation
namespace: oat_trait_method
def: "Observe relative or absolute area of plant tissue affected by Stem rust and record it. Often severity is represented as a proportion or percentage of plant surface affected." []
relationship: method_of CO_350:0000114

[Term]
id: CO_350:0000046
name: DON concentration determination
namespace: oat_trait_method
def: "Computation of the deoxynivalenol content" []
relationship: method_of CO_350:0000045

[Term]
id: CO_350:0000034
name: Avenanthramide content determination
namespace: oat_trait_method
def: "Direct measurement of the total avenanthramide content" []
relationship: method_of CO_350:0000033

[Term]
id: CO_350:0005601
name: Freeze damage severity observation
namespace: oat_trait_method
def: "Estimation of the freeze damage severity using a 0-9 scale: 0= no freeze damage, 9= severe freeze damage." []
relationship: method_of CO_350:0005401

[Term]
id: CO_350:0005602
name: Storm damage severity observation
namespace: oat_trait_method
def: "Estimation of the storm damage severity using a 1-5 scale: 1= no damage, 5= total damage and loss of plot." []
relationship: method_of CO_350:0005402

[Term]
id: CO_350:0005603
name: Winter stress severity observation
namespace: oat_trait_method
def: "Estimation of the winter stress severity using a 0-9 scale: 0= no signs of winter stress, 9= severe leaf damage or leaves that are purple in color.	" []
relationship: method_of CO_350:0005403

[Term]
id: CO_350:0005604
name: Emergence measurement
namespace: oat_trait_method
def: "Measurement of the percentage of plants in a plot that have emerged" []
relationship: method_of CO_350:0005404

[Term]
id: CO_350:0005605
name: Forage rating estimation
namespace: oat_trait_method
def: "Estimation of the forage rating using a 0-9 scale: 0= low, 9= high" []
relationship: method_of CO_350:0005405

[Term]
id: CO_350:0005606
name: Groat content determination (hand dehulled)
namespace: oat_trait_method
def: "Calculated as the total groat weight divided by the initial kernel weight before dehulling, multiplied by 100. Kernels are dehulled by hand and sample sizes are smaller than for machine dehulling, for example two grams." []
relationship: method_of CO_350:0000009

[Term]
id: CO_350:0005607
name: Phenotype score observation
namespace: oat_trait_method
def: "Visual assessment of the phenotype score using a 0-9 scale: 0= perfect, 1= excellent, 4= good, 5= borderline, 6= poor, 9= unadapted" []
relationship: method_of CO_350:0005406

[Term]
id: CO_350:0005608
name: Silage yield 65% moisture determination
namespace: oat_trait_method
def: "Silage yield at 65% moisture content" []
relationship: method_of CO_350:0005407

[Term]
id: CO_350:0005609
name: Silage yield dry matter determination
namespace: oat_trait_method
def: "Yield of dry matter for use as silage" []
relationship: method_of CO_350:0005407

[Term]
id: CO_350:0005610
name: BYDV severity estimation
namespace: oat_trait_method
def: "Estimation of the severity of barley yellow dwarf virus symptoms observed in a plot; plots rated 0 exhibit essentially no chlorosis, no stunted tillers, and no blasting, plots rated 9 do not head and are very severely stunted." []
relationship: method_of CO_350:0000084

[Term]
id: CO_350:0005611
name: Bird damage severity observation
namespace: oat_trait_method
def: "Estimation of the severity of the symptoms of bird damage on a 0-9 scale: 0= no bird damage, 9= severe bird damage" []
relationship: method_of CO_350:0005408

[Term]
id: CO_350:0005612
name: Cereal leaf beetle damage severity observation
namespace: oat_trait_method
def: "Estimation of the severity of cereal leaf beetle damage on a 0-3 scale: 0= no larval feeding, 1= 1-15% foliage eaten, 2= 15-40% foliage eaten, 3= over 40% foliage eaten" []
relationship: method_of CO_350:0005409

[Term]
id: CO_350:0005613
name: Crown rust infection response estimation
namespace: oat_trait_method
def: "Estimation of the crown rust infection response. 	A qualitative analysis of the type of crown rust (Puccinia coronata f. sp. avenae) symptoms that are exhibited. Infection responses are limited to: Resistant (R): chlorotic fleck reaction with no sporulation; Moderately resistant (MR): Very small, non- or low-sporulating pustule surrounded by chlorosis; Moderately susceptible (MS): moderate to large pustule surrounded by extensive chlorosis, and; Susceptible (S): large pustule with little or no chlorosis. The following numerical scale has been used to quantify conventional notations of infection type: R= 0.2, R-MR= 0.3, MR= 0.4, R-MS= 0.45, R-S= 0.5, MR-MS= 0.6, MR-S= 0.7, MS= 0.8, MS-S= 0.9, S=1. Crown rust infection response is typically recorded in conjunction with crown rust severity." []
relationship: method_of CO_350:0000087

[Term]
id: CO_350:0005614
name: Crown rust infection type seedling BQBC
namespace: oat_trait_method
def: "A qualitative analysis of the type of disease symptoms exhibited by seedlings inoculated with crown rust (Puccinia coronata f. sp. avenae) race BQBC during greenhouse trials. Ratings made using the scale from Murphy (1935); immune/nearly immune= 0, highly resistant= 1, moderately resistant= 2, moderately susceptible= 3, and completely susceptible= 4." []
relationship: method_of CO_350:0000087

[Term]
id: CO_350:0005615
name: Crown rust infection type seedling BRBG-94
namespace: oat_trait_method
def: "A qualitative analysis of the type of disease symptoms exhibited by seedlings inoculated with crown rust (Puccinia coronata f. sp. avenae) race BRBG-94 during greenhouse trials. Ratings made using the scale from Murphy (1935); immune/nearly immune= 0, highly resistant= 1, moderately resistant= 2, moderately susceptible= 3, and completely susceptible= 4." []
relationship: method_of CO_350:0000087

[Term]
id: CO_350:0005616
name: Crown rust infection type seedling composite/unknown
namespace: oat_trait_method
def: "A qualitative analysis of the type of disease symptoms exhibited by seedlings inoculated with crown rust (Puccinia coronata f. sp. avenae) composite race / unknown race during greenhouse trials. Ratings made using the scale from Murphy (1935); immune/nearly immune= 0, highly resistant= 1, moderately resistant= 2, moderately susceptible= 3, and completely susceptible= 4." []
relationship: method_of CO_350:0000087

[Term]
id: CO_350:0005617
name: Crown rust infection type seedling DQBB
namespace: oat_trait_method
def: "A qualitative analysis of the type of disease symptoms exhibited by seedlings inoculated with crown rust (Puccinia coronata f. sp. avenae) race DQBB during greenhouse trials. Ratings made using the scale from Murphy (1935); immune/nearly immune= 0, highly resistant= 1, moderately resistant= 2, moderately susceptible= 3, and completely susceptible= 4." []
relationship: method_of CO_350:0000087

[Term]
id: CO_350:0005618
name: Crown rust infection type seedling DQBG
namespace: oat_trait_method
def: "A qualitative analysis of the type of disease symptoms exhibited by seedlings inoculated with crown rust (Puccinia coronata f. sp. avenae) race DQBG during greenhouse trials. Ratings made using the scale from Murphy (1935); immune/nearly immune= 0, highly resistant= 1, moderately resistant= 2, moderately susceptible= 3, and completely susceptible= 4." []
relationship: method_of CO_350:0000087

[Term]
id: CO_350:0005619
name: Crown rust infection type seedling DSGB
namespace: oat_trait_method
def: "A qualitative analysis of the type of disease symptoms exhibited by seedlings inoculated with crown rust (Puccinia coronata f. sp. avenae) race DSGB during greenhouse trials. Ratings made using the scale from Murphy (1935); immune/nearly immune= 0, highly resistant= 1, moderately resistant= 2, moderately susceptible= 3, and completely susceptible= 4." []
relationship: method_of CO_350:0000087

[Term]
id: CO_350:0005620
name: Crown rust infection type seedling LQCB-91
namespace: oat_trait_method
def: "A qualitative analysis of the type of disease symptoms exhibited by seedlings inoculated with crown rust (Puccinia coronata f. sp. avenae) race LQCB-91 during greenhouse trials. Ratings made using the scale from Murphy (1935); immune/nearly immune= 0, highly resistant= 1, moderately resistant= 2, moderately susceptible= 3, and completely susceptible= 4." []
relationship: method_of CO_350:0000087

[Term]
id: CO_350:0005621
name: Crown rust infection type seedling LRBG
namespace: oat_trait_method
def: "A qualitative analysis of the type of disease symptoms exhibited by seedlings inoculated with crown rust (Puccinia coronata f. sp. avenae) race LRBG during greenhouse trials. Ratings made using the scale from Murphy (1935); immune/nearly immune= 0, highly resistant= 1, moderately resistant= 2, moderately susceptible= 3, and completely susceptible= 4." []
relationship: method_of CO_350:0000087

[Term]
id: CO_350:0005622
name: Crown rust infection type seedling MHBB
namespace: oat_trait_method
def: "A qualitative analysis of the type of disease symptoms exhibited by seedlings inoculated with crown rust (Puccinia coronata f. sp. avenae) race MHBB during greenhouse trials. Ratings made using the scale from Murphy (1935); immune/nearly immune= 0, highly resistant= 1, moderately resistant= 2, moderately susceptible= 3, and completely susceptible= 4." []
relationship: method_of CO_350:0000087

[Term]
id: CO_350:0005623
name: Crown rust infection type seedling NBFB
namespace: oat_trait_method
def: "A qualitative analysis of the type of disease symptoms exhibited by seedlings inoculated with crown rust (Puccinia coronata f. sp. avenae) race NBFB during greenhouse trials. Ratings made using the scale from Murphy (1935); immune/nearly immune= 0, highly resistant= 1, moderately resistant= 2, moderately susceptible= 3, and completely susceptible= 4." []
relationship: method_of CO_350:0000087

[Term]
id: CO_350:0005624
name: Crown rust infection type seedling NGCC-94
namespace: oat_trait_method
def: "A qualitative analysis of the type of disease symptoms exhibited by seedlings inoculated with crown rust (Puccinia coronata f. sp. avenae) race NGCC-94 during greenhouse trials. Ratings made using the scale from Murphy (1935); immune/nearly immune= 0, highly resistant= 1, moderately resistant= 2, moderately susceptible= 3, and completely susceptible= 4." []
relationship: method_of CO_350:0000087

[Term]
id: CO_350:0005625
name: Crown rust infection type seedling NQBB
namespace: oat_trait_method
def: "A qualitative analysis of the type of disease symptoms exhibited by seedlings inoculated with crown rust (Puccinia coronata f. sp. avenae) race NQBB during greenhouse trials. Ratings made using the scale from Murphy (1935); immune/nearly immune= 0, highly resistant= 1, moderately resistant= 2, moderately susceptible= 3, and completely susceptible= 4." []
relationship: method_of CO_350:0000087

[Term]
id: CO_350:0005626
name: Crown rust infection type seedling NTGG
namespace: oat_trait_method
def: "A qualitative analysis of the type of disease symptoms exhibited by seedlings inoculated with crown rust (Puccinia coronata f. sp. avenae) race NTGG during greenhouse trials. Ratings made using the scale from Murphy (1935); immune/nearly immune= 0, highly resistant= 1, moderately resistant= 2, moderately susceptible= 3, and completely susceptible= 4." []
relationship: method_of CO_350:0000087

[Term]
id: CO_350:0005627
name: Crown rust infection type seedling SJGL
namespace: oat_trait_method
def: "A qualitative analysis of the type of disease symptoms exhibited by seedlings inoculated with crown rust (Puccinia coronata f. sp. avenae) race SJGL during greenhouse trials. Ratings made using the scale from Murphy (1935); immune/nearly immune= 0, highly resistant= 1, moderately resistant= 2, moderately susceptible= 3, and completely susceptible= 4." []
relationship: method_of CO_350:0000087

[Term]
id: CO_350:0005628
name: Crown rust flag leaf severity estimation
namespace: oat_trait_method
def: "Estimation of the percentage of the area of the flag leaf occupied by crown rust (Puccinia coronata f. sp. avenae) pustules or necrosis, following the modified Cobb scale (Peterson et al. 1948) and recorded in conjunction with crown rust infection response. Common intervals: trace (0.1 in T3), 5, 10, 20, 40, 60, and 100 percent infection." []
relationship: method_of CO_350:0000090

[Term]
id: CO_350:0005629
name: Crown rust plot severity estimation
namespace: oat_trait_method
def: "Estimation of the severity of crown rust (Puccinia coronata f. sp. avenae) symptoms observed in a plot; plots rated 0 exhibit no symptoms, plots rated 9 show severe symptoms." []
relationship: method_of CO_350:0000090

[Term]
id: CO_350:0005630
name: Crown rust plant severity estimation
namespace: oat_trait_method
def: "Estimation of the severity of crown rust (Puccinia coronata f. sp. avenae) symptoms. Ratings based on the percent infection of the whole plant; 79-100%= 1, 90-97%= 2, 75-90%= 3, 60-75%= 4, 40-60%= 5, 25-40%= 6, 10-25%= 7, 3-10%= 8, 0-3%= 9." []
relationship: method_of CO_350:0000090

[Term]
id: CO_350:0005631
name: Downy mildew severity rating estimation
namespace: oat_trait_method
def: "Estimation of the severity of downy mildew (Sclerophthora macrospora) symptoms observed in a plot; plots rated 0 exhibit no symptoms, plots rated 9 show severe symptoms.	" []
relationship: method_of CO_350:0000523

[Term]
id: CO_350:0005632
name: Fusarium head blight incidence estimation
namespace: oat_trait_method
def: "Estimation of the incidence of Fusarium head blight (Fusarium spp.; FHB) symptoms observed in a plot; plots rated 0 exhibit no FHB symptoms, plots rated 1 contain a few blighted spikelets, while a rating of 4 indicates that the whole plot is blighted." []
relationship: method_of CO_350:0000093

[Term]
id: CO_350:0005633
name: Stagonospora severity estimation
namespace: oat_trait_method
def: "Estimation of the severity Stagonospora avenae f. sp. avenaria symptoms in a plot using a 0-9 scale: 0= no symptoms, 9= high symptoms." []
relationship: method_of CO_350:0005410

[Term]
id: CO_350:0005634
name: Stem rust infection response estimation
namespace: oat_trait_method
def: "Estimation of the stem rust infection response. A qualitative analysis of the type of stem rust (Puccinia graminis f. sp. avenae) symptoms that are exhibited. Infection responses are limited to: Resistant (R): chlorotic fleck reaction with no sporulation; Moderately resistant (MR): Very small, non- or low-sporulating pustule surrounded by chlorosis; Moderately susceptible (MS): moderate to large pustule surrounded by extensive chlorosis, and; Susceptible (S): large pustule with little or no chlorosis. The following numerical scale has been used to quantify conventional notations of infection type: R= 0.2, R-MR= 0.3, MR= 0.4, R-MS= 0.45, R-S= 0.5, MR-MS= 0.6, MR-S= 0.7, MS= 0.8, MS-S= 0.9, S=1. Stem rust infection response is typically recorded in conjunction with stem rust severity." []
relationship: method_of CO_350:0000111

[Term]
id: CO_350:0005635
name: Stem rust infection type seedling composite/unknown
namespace: oat_trait_method
def: "A qualitative analysis of the type of disease symptoms exhibited by seedlings inoculated with a composite collection or unknown race of stem rust (Puccinia graminis f. sp. avenae) during greenhouse trials. Ratings made using the scale from Stakman et al. (1962); immune= 0, very resistant= 1, moderately resistant= 2, moderately susceptible= 3, and very susceptible= 4." []
relationship: method_of CO_350:0000111

[Term]
id: CO_350:0005636
name: Stem rust infection type seedling NA1
namespace: oat_trait_method
def: "A qualitative analysis of the type of disease symptoms exhibited by seedlings inoculated with stem rust (Puccinia graminis f. sp. avenae) race NA1 during greenhouse trials. Ratings made using the scale from Stakman et al. (1962); immune= 0, very resistant= 1, moderately resistant= 2, moderately susceptible= 3, and very susceptible= 4. " []
relationship: method_of CO_350:0000111

[Term]
id: CO_350:0005637
name: Stem rust infection type seedling NA16
namespace: oat_trait_method
def: "A qualitative analysis of the type of disease symptoms exhibited by seedlings inoculated with stem rust (Puccinia graminis f. sp. avenae) race NA16 during greenhouse trials. Ratings made using the scale from Stakman et al. (1962); immune= 0, very resistant= 1, moderately resistant= 2, moderately susceptible= 3, and very susceptible= 4. " []
relationship: method_of CO_350:0000111

[Term]
id: CO_350:0005638
name: Stem rust infection type seedling NA25
namespace: oat_trait_method
def: "A qualitative analysis of the type of disease symptoms exhibited by seedlings inoculated with stem rust (Puccinia graminis f. sp. avenae) race NA25 during greenhouse trials. Ratings made using the scale from Stakman et al. (1962); immune= 0, very resistant= 1, moderately resistant= 2, moderately susceptible= 3, and very susceptible= 4. " []
relationship: method_of CO_350:0000111

[Term]
id: CO_350:0005639
name: Stem rust infection type seedling NA27
namespace: oat_trait_method
def: "A qualitative analysis of the type of disease symptoms exhibited by seedlings inoculated with stem rust (Puccinia graminis f. sp. avenae) race NA27 during greenhouse trials. Ratings made using the scale from Stakman et al. (1962); immune= 0, very resistant= 1, moderately resistant= 2, moderately susceptible= 3, and very susceptible= 4. " []
relationship: method_of CO_350:0000111

[Term]
id: CO_350:0005640
name: Stem rust infection type seedling NA28
namespace: oat_trait_method
def: "A qualitative analysis of the type of disease symptoms exhibited by seedlings inoculated with stem rust (Puccinia graminis f. sp. avenae) race NA28 during greenhouse trials. Ratings made using the scale from Stakman et al. (1962); immune= 0, very resistant= 1, moderately resistant= 2, moderately susceptible= 3, and very susceptible= 4. " []
relationship: method_of CO_350:0000111

[Term]
id: CO_350:0005641
name: Stem rust infection type seedling NA29
namespace: oat_trait_method
def: "A qualitative analysis of the type of disease symptoms exhibited by seedlings inoculated with stem rust (Puccinia graminis f. sp. avenae) race NA29 during greenhouse trials. Ratings made using the scale from Stakman et al. (1962); immune= 0, very resistant= 1, moderately resistant= 2, moderately susceptible= 3, and very susceptible= 4. " []
relationship: method_of CO_350:0000111

[Term]
id: CO_350:0005642
name: Stem rust infection type seedling NA55
namespace: oat_trait_method
def: "A qualitative analysis of the type of disease symptoms exhibited by seedlings inoculated with stem rust (Puccinia graminis f. sp. avenae) race NA55 during greenhouse trials. Ratings made using the scale from Stakman et al. (1962); immune= 0, very resistant= 1, moderately resistant= 2, moderately susceptible= 3, and very susceptible= 4. " []
relationship: method_of CO_350:0000111

[Term]
id: CO_350:0005643
name: Stem rust infection type seedling NA67
namespace: oat_trait_method
def: "A qualitative analysis of the type of disease symptoms exhibited by seedlings inoculated with stem rust (Puccinia graminis f. sp. avenae) race NA67 during greenhouse trials. Ratings made using the scale from Stakman et al. (1962); immune= 0, very resistant= 1, moderately resistant= 2, moderately susceptible= 3, and very susceptible= 4. " []
relationship: method_of CO_350:0000111

[Term]
id: CO_350:0005644
name: Stem rust infection type seedling NA8
namespace: oat_trait_method
def: "A qualitative analysis of the type of disease symptoms exhibited by seedlings inoculated with stem rust (Puccinia graminis f. sp. avenae) race NA8 during greenhouse trials. Ratings made using the scale from Stakman et al. (1962); immune= 0, very resistant= 1, moderately resistant= 2, moderately susceptible= 3, and very susceptible= 4. " []
relationship: method_of CO_350:0000111

[Term]
id: CO_350:0005645
name: Stem rust severity plot estimation
namespace: oat_trait_method
def: "Estimation of the severity of stem rust (Puccinia graminis f. sp. avenae) symptoms observed in a plot; plots rated 0 exhibit no symptoms, plots rated 9 show severe symptoms." []
relationship: method_of CO_350:0000114

[Term]
id: CO_350:0005646
name: GC-MS measurement
namespace: oat_trait_method
def: "Direct measurement of a gas chromatography mass spectrum" []
relationship: method_of CO_350:0005411

[Term]
id: CO_350:0005647
name: LC-MS measurement
namespace: oat_trait_method
def: "Direct measurement of a liquid chromatography mass spectrum" []
relationship: method_of CO_350:0005412

[Term]
id: CO_350:0005648
name: Grain plumpness 5.0/64 plump measurement
namespace: oat_trait_method
def: "Measurement of the percentage of grain that did not pass through a 5.0/64" sieve." []
relationship: method_of CO_350:0000066

[Term]
id: CO_350:0005649
name: Grain plumpness 5.0/64 thin measurement
namespace: oat_trait_method
def: "Measurement of the percentage of grain that passed through a 5.0/64" sieve." []
relationship: method_of CO_350:0000066

[Term]
id: CO_350:0005650
name: Grain plumpness 5.5/64 plump measurement
namespace: oat_trait_method
def: "Measurement of the percentage of grain that did not pass through a 5.5/64" sieve." []
relationship: method_of CO_350:0000066

[Term]
id: CO_350:0005651
name: Growth habit estimation
namespace: oat_trait_method
def: "A visual assessment of the growth habit:  very upright spring type= 0, very prostrate winter type= 9." []
relationship: method_of CO_350:0005413

[Term]
id: CO_350:0005652
name: Hull color estimation
namespace: oat_trait_method
def: "A visual assessment of the hull color using a 1-10 rating: white= 1, cream= 2, light tan= 3, yellow= 6, black= 10." []
relationship: method_of CO_350:0005414

[Term]
id: CO_350:0005653
name: Kernels per spikelet estimation - 5 spikelets
namespace: oat_trait_method
def: "Calculation of the average number of kernels per spikelet, based on five typical spikelets." []
relationship: method_of CO_350:0005415

[Term]
id: CO_350:0005654
name: Leaf biomass estimation
namespace: oat_trait_method
def: "Estimation of the leaf biomass as a 'leafiness' rating on a 0-9 scale: very leafy= 3, few leaves=9." []
relationship: method_of CO_350:0005416

[Term]
id: CO_350:0005655
name: Panicle length estimation - 5 panicles
namespace: oat_trait_method
def: "Calculation of the average panicle length from five mature panicles measured from the lowest panicle node to the tip of the apical spike" []
relationship: method_of CO_350:0005417

[Term]
id: CO_350:0005656
name: Spikelets per panicle estimation - 5 panicles
namespace: oat_trait_method
def: "Calculation of the average number of spikelets per panicle, based on five mature panicles" []
relationship: method_of CO_350:0005418

[Term]
id: CO_350:0005657
name: Avenanthramide 2c content determination
namespace: oat_trait_method
def: "Direct measurement of the avenanthramide 2c content" []
relationship: method_of CO_350:0000033

[Term]
id: CO_350:0005658
name: Avenanthramide 2f content determination
namespace: oat_trait_method
def: "Direct measurement of the avenanthramide 2f content" []
relationship: method_of CO_350:0000033

[Term]
id: CO_350:0005659
name: Avenanthramide 2p content determination
namespace: oat_trait_method
def: "Direct measurement of the avenanthramide 2p content" []
relationship: method_of CO_350:0000033

[Term]
id: CO_350:0005660
name: Avenanthramide 5p content determination
namespace: oat_trait_method
def: "Direct measurement of the avenanthramide 5p content" []
relationship: method_of CO_350:0000033

[Term]
id: CO_350:0005661
name: Avenanthramide A relative abundance estimation
namespace: oat_trait_method
def: "Estimation of the avenanthramide A relative abundance by UPLC" []
relationship: method_of CO_350:0005419

[Term]
id: CO_350:0005662
name: Avenanthramide B relative abundance estimation
namespace: oat_trait_method
def: "Estimation of the avenanthramide B relative abundance by UPLC" []
relationship: method_of CO_350:0005419

[Term]
id: CO_350:0005663
name: Avenanthramide C relative abundance estimation
namespace: oat_trait_method
def: "Estimation of the avenanthramide C relative abundance by UPLC" []
relationship: method_of CO_350:0005419

[Term]
id: CO_350:0005664
name: Beta-glucan content NIRS determination
namespace: oat_trait_method
def: "Measurement of beta-glucan content obtained using near-infrared spectroscopy (NIR)." []
relationship: method_of CO_350:0000036

[Term]
id: CO_350:0005665
name: Dehulling efficiency computation
namespace: oat_trait_method
def: "Computation of the percentage of seed that is effectively dehulled by a Codema dehuller; calculated as the mass of seed before dehulling minus the amount of undehulled seed after processing, divided by the total mass before dehulling, and multiplied by 100 to give the percentage of seed that was successfully dehulled." []
relationship: method_of CO_350:0005420

[Term]
id: CO_350:0005666
name: Dietary fiber content determination - HMW / ethanol-insoluble
namespace: oat_trait_method
def: "Computation of the ethanol-insoluble high molecular weight dietary fiber content; measured on a dry weight basis using wet chemistry." []
relationship: method_of CO_350:0000042

[Term]
id: CO_350:0005667
name: Dietary fiber content determination - HMW / ethanol-soluble
namespace: oat_trait_method
def: "Computation of the ethanol-soluble high molecular weight dietary fiber content; measured on a dry weight basis using wet chemistry." []
relationship: method_of CO_350:0000042

[Term]
id: CO_350:0005668
name: Dietary fiber content determiation - HMW
namespace: oat_trait_method
def: "Computation of the high molecular weight dietary fiber content; measured on a dry weight basis using wet chemistry." []
relationship: method_of CO_350:0000042

[Term]
id: CO_350:0005669
name: Dietary fiber content determination - LMW
namespace: oat_trait_method
def: "Computation of the low molecular weight dietary fiber content; measured on a dry weight basis using wet chemistry." []
relationship: method_of CO_350:0000042

[Term]
id: CO_350:0005670
name: DON 3-acetyl concentration determination
namespace: oat_trait_method
def: "Computation of the 3-acetyl-deoxynivalenol content" []
relationship: method_of CO_350:0005421

[Term]
id: CO_350:0005671
name: Fatty acid C14:0 content measurement
namespace: oat_trait_method
def: "Measurement of fatty acid C14:0 content" []
relationship: method_of CO_350:0005422

[Term]
id: CO_350:0005672
name: Fatty acid C16:0 content measurement
namespace: oat_trait_method
def: "Measurement of fatty acid C16:0 content" []
relationship: method_of CO_350:0005422

[Term]
id: CO_350:0005673
name: Fatty acid C16:1 content measurement
namespace: oat_trait_method
def: "Measurement of fatty acid C16:1 content" []
relationship: method_of CO_350:0005422

[Term]
id: CO_350:0005674
name: Fatty acid C18:0 content measurement
namespace: oat_trait_method
def: "Measurement of fatty acid C18:0 content" []
relationship: method_of CO_350:0005422

[Term]
id: CO_350:0005675
name: Fatty acid C18:1(9) content measurement
namespace: oat_trait_method
def: "Measurement of fatty acid C18:1(9) content" []
relationship: method_of CO_350:0005422

[Term]
id: CO_350:0005676
name: Fatty acid C18:1* content measurement
namespace: oat_trait_method
def: "Measurement of fatty acid C18:1* content" []
relationship: method_of CO_350:0005422

[Term]
id: CO_350:0005677
name: Fatty acid C18:2 content measurement
namespace: oat_trait_method
def: "Measurement of fatty acid C18:2 content" []
relationship: method_of CO_350:0005422

[Term]
id: CO_350:0005678
name: Fatty acid C18:3 content measurement
namespace: oat_trait_method
def: "Measurement of fatty acid C18:3 content" []
relationship: method_of CO_350:0005422

[Term]
id: CO_350:0005679
name: Fatty acid C19:0 content measurement
namespace: oat_trait_method
def: "Measurement of fatty acid C19:0 content" []
relationship: method_of CO_350:0005422

[Term]
id: CO_350:0005680
name: Fatty acid C20:0 content measurement
namespace: oat_trait_method
def: "Measurement of fatty acid C20:0 content" []
relationship: method_of CO_350:0005422

[Term]
id: CO_350:0005681
name: Fatty acid C20:1 content measurement
namespace: oat_trait_method
def: "Measurement of fatty acid C20:1 content" []
relationship: method_of CO_350:0005422

[Term]
id: CO_350:0005682
name: Groat flour falling number determination
namespace: oat_trait_method
def: "Measurement of the amount of time it takes for a viscometer stirrer to fall a set distance through an aqueous gel created using groat flour. This indirectly measures the alpha amylase content of the groat, which becomes more abundant in grains that have suffered pre-harvest sprouting. An increase in alpha amylase in groat flour, along with other hydrolytic enzymes that are associated with pre-harvest sprouting, reduces the quality of the flour." []
relationship: method_of CO_350:0005423

[Term]
id: CO_350:0005683
name: Lutein content measurement
namespace: oat_trait_method
def: "Measurement of the lutein content" []
relationship: method_of CO_350:0005424

[Term]
id: CO_350:0005684
name: Phytoene content measurement
namespace: oat_trait_method
def: "Measurement of the phytoene content" []
relationship: method_of CO_350:0005425

[Term]
id: CO_350:0005685
name: Phytofluene content measurement
namespace: oat_trait_method
def: "Measurement of the phytofluene content" []
relationship: method_of CO_350:0005426

[Term]
id: CO_350:0005686
name: Seed quality estimation
namespace: oat_trait_method
def: "Estimation of the seed qulaity on a 1-7 scale: 1= excellent, 7= poor" []
relationship: method_of CO_350:0005427

[Term]
id: CO_350:0005687
name: Silage moisture content determination
namespace: oat_trait_method
def: "Measurement of the moisture content of silage." []
relationship: method_of CO_350:0005428

[Term]
id: CO_350:0005688
name: Total toco content determination
namespace: oat_trait_method
def: "Measurement of the total -tocopherol and -tocotrienol content" []
relationship: method_of CO_350:0005429

[Term]
id: CO_350:0005689
name: Alpha-tocopherol content determination
namespace: oat_trait_method
def: "Measurement of the alpha-tocopherol content" []
relationship: method_of CO_350:0000060

[Term]
id: CO_350:0005690
name: Beta-tocopherol content determination
namespace: oat_trait_method
def: "Measurement of the beta-tocopherol content" []
relationship: method_of CO_350:0000060

[Term]
id: CO_350:0005691
name: Delta-tocopherol content determination
namespace: oat_trait_method
def: "Measurement of the delta-tocopherol content" []
relationship: method_of CO_350:0000060

[Term]
id: CO_350:0005692
name: Gamma-tocopherol content determination
namespace: oat_trait_method
def: "Measurement of the gamma-tocopherol content" []
relationship: method_of CO_350:0000060

[Term]
id: CO_350:0005693
name: Alpha-tocotrienol content determination
namespace: oat_trait_method
def: "Measurement of the alpha-tocotrienol content" []
relationship: method_of CO_350:0000057

[Term]
id: CO_350:0005694
name: Beta-tocotrienol content determination
namespace: oat_trait_method
def: "Measurement of the beta-tocotrienol content" []
relationship: method_of CO_350:0000057

[Term]
id: CO_350:0005695
name: Delta-tocotrienol content determination
namespace: oat_trait_method
def: "Measurement of the delta-tocotrienol content" []
relationship: method_of CO_350:0000057

[Term]
id: CO_350:0005696
name: Gamma-tocotrienol content determination
namespace: oat_trait_method
def: "Measurement of the gamma-tocotrienol content" []
relationship: method_of CO_350:0000057

[Term]
id: CO_350:0005697
name: Tunaxanthin content determination
namespace: oat_trait_method
def: "Measurement of the tunaxanthin content" []
relationship: method_of CO_350:0005430

[Term]
id: CO_350:0005698
name: Violaxanthin content determination
namespace: oat_trait_method
def: "Measurement of the Violaxanthin content" []
relationship: method_of CO_350:0005431

[Term]
id: CO_350:0005699
name: Zeaxanthin content determination
namespace: oat_trait_method
def: "Measurement of the Zeaxanthin content" []
relationship: method_of CO_350:0005432

[Term]
id: CO_350:0000011
name: percent
namespace: oat_trait_scale
relationship: scale_of CO_350:0005684
relationship: scale_of CO_350:0005673
relationship: scale_of CO_350:0000049
relationship: scale_of CO_350:0005666
relationship: scale_of CO_350:0005677
relationship: scale_of CO_350:0005664
relationship: scale_of CO_350:0005675
relationship: scale_of CO_350:0000043
relationship: scale_of CO_350:0000010
relationship: scale_of CO_350:0005665
relationship: scale_of CO_350:0005676
relationship: scale_of CO_350:0005699
relationship: scale_of CO_350:0000626
relationship: scale_of CO_350:0005606
relationship: scale_of CO_350:0005604
relationship: scale_of CO_350:0005650
relationship: scale_of CO_350:0000082
relationship: scale_of CO_350:0000055
relationship: scale_of CO_350:0005681
relationship: scale_of CO_350:0005648
relationship: scale_of CO_350:0005671
relationship: scale_of CO_350:0005698
relationship: scale_of CO_350:0000031
relationship: scale_of CO_350:0005687
relationship: scale_of CO_350:0005649
relationship: scale_of CO_350:0000573
relationship: scale_of CO_350:0005667
relationship: scale_of CO_350:0005669
relationship: scale_of CO_350:0005668
relationship: scale_of CO_350:0005680
relationship: scale_of CO_350:0005679
relationship: scale_of CO_350:0005697
relationship: scale_of CO_350:0005678
relationship: scale_of CO_350:0005674
relationship: scale_of CO_350:0000037
relationship: scale_of CO_350:0005683
relationship: scale_of CO_350:0005672
relationship: scale_of CO_350:0000016
relationship: scale_of CO_350:0000040
relationship: scale_of CO_350:0005628
relationship: scale_of CO_350:0005685
relationship: scale_of CO_350:0000052
relationship: scale_of CO_350:0000535

[Term]
id: CO_350:0000086
name: 0-9 disease severity scale
namespace: oat_trait_scale
relationship: scale_of CO_350:0000085

[Term]
id: CO_350:0000005
name: 1-10 breakage incidence scale
namespace: oat_trait_scale
relationship: scale_of CO_350:0000004

[Term]
id: CO_350:0000071
name: 1-10 grain color scale
namespace: oat_trait_scale
def: "1= white, 2= cream, 3= light tan, 6= yellow, 10= black" []
relationship: scale_of CO_350:0005652

[Term]
id: CO_350:0000071/0
name: white
namespace: oat_trait_scale
synonym: "1" EXACT []
is_a: CO_350:0000071

[Term]
id: CO_350:0000071/1
name: cream
namespace: oat_trait_scale
synonym: "2" EXACT []
is_a: CO_350:0000071

[Term]
id: CO_350:0000071/2
name: light tan
namespace: oat_trait_scale
synonym: "3" EXACT []
is_a: CO_350:0000071

[Term]
id: CO_350:0000071/3
name: yellow
namespace: oat_trait_scale
synonym: "6" EXACT []
is_a: CO_350:0000071

[Term]
id: CO_350:0000071/4
name: black
namespace: oat_trait_scale
synonym: "10" EXACT []
is_a: CO_350:0000071

[Term]
id: CO_350:0000074
name: 1-4 groat color scale
namespace: oat_trait_scale
def: "1= light red, 2= light brown, 3= medium brown, 4= dark brown" []
relationship: scale_of CO_350:0000073

[Term]
id: CO_350:0000074/0
name: light red
namespace: oat_trait_scale
synonym: "1" EXACT []
is_a: CO_350:0000074

[Term]
id: CO_350:0000074/1
name: light brown
namespace: oat_trait_scale
synonym: "2" EXACT []
is_a: CO_350:0000074

[Term]
id: CO_350:0000074/2
name: medium brown
namespace: oat_trait_scale
synonym: "3" EXACT []
is_a: CO_350:0000074

[Term]
id: CO_350:0000074/3
name: dark brown
namespace: oat_trait_scale
synonym: "4" EXACT []
is_a: CO_350:0000074

[Term]
id: CO_350:0000002
name: 1-5 agronomic score scale
namespace: oat_trait_scale
relationship: scale_of CO_350:0000001

[Term]
id: CO_350:0000026
name: 1-9 relative canopy development scale
namespace: oat_trait_scale
relationship: scale_of CO_350:0000025

[Term]
id: CO_350:0000029
name: 1-9 snapback scale
namespace: oat_trait_scale
relationship: scale_of CO_350:0000028

[Term]
id: CO_350:0000023
name: cm
namespace: oat_trait_scale
relationship: scale_of CO_350:0005655
relationship: scale_of CO_350:0000022

[Term]
id: CO_350:0000249
name: g
namespace: oat_trait_scale
relationship: scale_of CO_350:0000064
relationship: scale_of CO_350:0000079

[Term]
id: CO_350:0000077
name: g/L
namespace: oat_trait_scale
relationship: scale_of CO_350:0000076

[Term]
id: CO_350:0000008
name: g/m2
namespace: oat_trait_scale
relationship: scale_of CO_350:0000007

[Term]
id: CO_350:0000014
name: Julian day
namespace: oat_trait_scale
relationship: scale_of CO_350:0000019
relationship: scale_of CO_350:0000013

[Term]
id: CO_350:0000047
name: ppm
namespace: oat_trait_scale
relationship: scale_of CO_350:0005670
relationship: scale_of CO_350:0000046

[Term]
id: CO_350:0000035
name: ug/g
namespace: oat_trait_scale
relationship: scale_of CO_350:0005658
relationship: scale_of CO_350:0005691
relationship: scale_of CO_350:0005657
relationship: scale_of CO_350:0005689
relationship: scale_of CO_350:0005693
relationship: scale_of CO_350:0005692
relationship: scale_of CO_350:0005694
relationship: scale_of CO_350:0005659
relationship: scale_of CO_350:0005688
relationship: scale_of CO_350:0005696
relationship: scale_of CO_350:0005695
relationship: scale_of CO_350:0000034
relationship: scale_of CO_350:0005690
relationship: scale_of CO_350:0005660

[Term]
id: CO_350:0005901
name: 0-9 rating scale
namespace: oat_trait_scale
relationship: scale_of CO_350:0005607
relationship: scale_of CO_350:0005629
relationship: scale_of CO_350:0005601
relationship: scale_of CO_350:0005654
relationship: scale_of CO_350:0005610
relationship: scale_of CO_350:0000118
relationship: scale_of CO_350:0005651
relationship: scale_of CO_350:0005633
relationship: scale_of CO_350:0005645
relationship: scale_of CO_350:0005611
relationship: scale_of CO_350:0005631
relationship: scale_of CO_350:0005605
relationship: scale_of CO_350:0005603

[Term]
id: CO_350:0005902
name: 1-5 rating scale
namespace: oat_trait_scale
relationship: scale_of CO_350:0005602

[Term]
id: CO_350:0005903
name: t/ac
namespace: oat_trait_scale
relationship: scale_of CO_350:0005608
relationship: scale_of CO_350:0005609

[Term]
id: CO_350:0005904
name: 1-3 rating scale
namespace: oat_trait_scale
relationship: scale_of CO_350:0005612

[Term]
id: CO_350:0005905
name: Disease Infection Response Rating (0-1)
namespace: oat_trait_scale
def: "0.2= R, 0.3= R-MR, 0.4= MR, 0.45= R-MS, 0.5= R-S, 0.6= MR-MS, 0.7= MR-S, 0.8= MS, 0.9= MS-S, 1.0= S" []
relationship: scale_of CO_350:0005613
relationship: scale_of CO_350:0005634

[Term]
id: CO_350:0005905/0
name: R
namespace: oat_trait_scale
synonym: "0.2" EXACT []
is_a: CO_350:0005905

[Term]
id: CO_350:0005905/1
name: R-MR
namespace: oat_trait_scale
synonym: "0.3" EXACT []
is_a: CO_350:0005905

[Term]
id: CO_350:0005905/2
name: MR
namespace: oat_trait_scale
synonym: "0.4" EXACT []
is_a: CO_350:0005905

[Term]
id: CO_350:0005905/3
name: R-MS
namespace: oat_trait_scale
synonym: "0.45" EXACT []
is_a: CO_350:0005905

[Term]
id: CO_350:0005905/4
name: R-S
namespace: oat_trait_scale
synonym: "0.5" EXACT []
is_a: CO_350:0005905

[Term]
id: CO_350:0005905/5
name: MR-MS
namespace: oat_trait_scale
synonym: "0.6" EXACT []
is_a: CO_350:0005905

[Term]
id: CO_350:0005905/6
name: MR-S
namespace: oat_trait_scale
synonym: "0.7" EXACT []
is_a: CO_350:0005905

[Term]
id: CO_350:0005905/7
name: MS
namespace: oat_trait_scale
synonym: "0.8" EXACT []
is_a: CO_350:0005905

[Term]
id: CO_350:0005905/8
name: MS-S
namespace: oat_trait_scale
synonym: "0.9" EXACT []
is_a: CO_350:0005905

[Term]
id: CO_350:0005905/9
name: S
namespace: oat_trait_scale
synonym: "1.0" EXACT []
is_a: CO_350:0005905

[Term]
id: CO_350:0005906
name: Murphy Infection Type Rating (0-4)
namespace: oat_trait_scale
def: "0= immune/nearly immune, 1= highly resistant, 2= moderately resistant, 3= moderately susceptible, 4= completely susceptible" []
relationship: scale_of CO_350:0005643
relationship: scale_of CO_350:0005644
relationship: scale_of CO_350:0005622
relationship: scale_of CO_350:0005616
relationship: scale_of CO_350:0005636
relationship: scale_of CO_350:0005615
relationship: scale_of CO_350:0005620
relationship: scale_of CO_350:0005624
relationship: scale_of CO_350:0005623
relationship: scale_of CO_350:0005638
relationship: scale_of CO_350:0005625
relationship: scale_of CO_350:0005617
relationship: scale_of CO_350:0005641
relationship: scale_of CO_350:0005619
relationship: scale_of CO_350:0005626
relationship: scale_of CO_350:0005627
relationship: scale_of CO_350:0005635
relationship: scale_of CO_350:0005637
relationship: scale_of CO_350:0005639
relationship: scale_of CO_350:0005614
relationship: scale_of CO_350:0005621
relationship: scale_of CO_350:0005618
relationship: scale_of CO_350:0005642
relationship: scale_of CO_350:0005640

[Term]
id: CO_350:0005906/0
name: immune/nearly immune
namespace: oat_trait_scale
synonym: "0" EXACT []
is_a: CO_350:0005906

[Term]
id: CO_350:0005906/1
name: highly resistant
namespace: oat_trait_scale
synonym: "1" EXACT []
is_a: CO_350:0005906

[Term]
id: CO_350:0005906/2
name: moderately resistant
namespace: oat_trait_scale
synonym: "2" EXACT []
is_a: CO_350:0005906

[Term]
id: CO_350:0005906/3
name: moderately susceptible
namespace: oat_trait_scale
synonym: "3" EXACT []
is_a: CO_350:0005906

[Term]
id: CO_350:0005906/4
name: completely susceptible
namespace: oat_trait_scale
synonym: "4" EXACT []
is_a: CO_350:0005906

[Term]
id: CO_350:0005907
name: 9-1 rating scale
namespace: oat_trait_scale
def: "9= low, 1= high" []
relationship: scale_of CO_350:0005630

[Term]
id: CO_350:0005907/0
name: low
namespace: oat_trait_scale
synonym: "9" EXACT []
is_a: CO_350:0005907

[Term]
id: CO_350:0005907/1
name: high
namespace: oat_trait_scale
synonym: "1" EXACT []
is_a: CO_350:0005907

[Term]
id: CO_350:0005908
name: 0-4 rating scale
namespace: oat_trait_scale
relationship: scale_of CO_350:0005632

[Term]
id: CO_350:0005909
name: mass spectrometry intensity
namespace: oat_trait_scale
relationship: scale_of CO_350:0005646
relationship: scale_of CO_350:0005647

[Term]
id: CO_350:0005910
name: kernels/spikelet
namespace: oat_trait_scale
relationship: scale_of CO_350:0005653

[Term]
id: CO_350:0005911
name: spikelets/panicle
namespace: oat_trait_scale
relationship: scale_of CO_350:0005656

[Term]
id: CO_350:0005912
name: relative abundance
namespace: oat_trait_scale
relationship: scale_of CO_350:0005661
relationship: scale_of CO_350:0005663
relationship: scale_of CO_350:0005662

[Term]
id: CO_350:0005913
name: seconds
namespace: oat_trait_scale
relationship: scale_of CO_350:0005682

[Term]
id: CO_350:0005914
name: 1-7 seed quality scale
namespace: oat_trait_scale
def: "1= excellent, 7= poor" []
relationship: scale_of CO_350:0005686

[Term]
id: CO_350:0005914/0
name: excellent
namespace: oat_trait_scale
synonym: "1" EXACT []
is_a: CO_350:0005914

[Term]
id: CO_350:0005914/1
name: poor
namespace: oat_trait_scale
synonym: "7" EXACT []
is_a: CO_350:0005914

[Term]
id: CO_350:0000155
name: Barley yellow dwarf virus incidence - percent
namespace: oat_trait
def: "TRAIT: Percentage of plants in a plot showing symptoms of barley yellow dwarf virus. METHOD: Visual assessment of the percentage of plants in a plot showing symptoms of a specific disease. SCALE: percent" []
relationship: variable_of CO_350:0000081
relationship: variable_of CO_350:0000082
relationship: variable_of CO_350:0000011

[Term]
id: CO_350:0000156
name: Beta-glucan content - dry weight basis - percent
namespace: oat_trait
def: "TRAIT: Amount of beta-glucan present in the groat expressed as a percentage of the entire groat. METHOD: Measurement of beta glucan content on a dry weight basis using a lichenase enzymatic procedure. SCALE: percent" []
relationship: variable_of CO_350:0000011
relationship: variable_of CO_350:0000037
relationship: variable_of CO_350:0000036

[Term]
id: CO_350:0000157
name: Broken groats - percent
namespace: oat_trait
def: "TRAIT: The amount of broken groats after de-hulling, expressed as a percentage of the weight of the entire whole grain sample. METHOD: Computation of the percentage of broken groats by weight after dehulling; calculated as the weight of broken groats divided by the total groat weight, multiplied by 100. SCALE: percent" []
relationship: variable_of CO_350:0000011
relationship: variable_of CO_350:0000040
relationship: variable_of CO_350:0000039

[Term]
id: CO_350:0000158
name: Dietary fiber content - total - percent
namespace: oat_trait
def: "TRAIT: Dietary fiber content METHOD: Computation of total dietary fiber content  on a dry weight basis using wet chemistry. SCALE: percent" []
relationship: variable_of CO_350:0000043
relationship: variable_of CO_350:0000042
relationship: variable_of CO_350:0000011

[Term]
id: CO_350:0000161
name: Grain protein content - percent
namespace: oat_trait
def: "TRAIT: The amount of protein in the grain, expressed as a percentage of the whole grain. METHOD: Computation of the percentage of protein in the whole grain as obtained using near-infrared spectroscopy (NIR). SCALE: percent" []
relationship: variable_of CO_350:0000048
relationship: variable_of CO_350:0000049
relationship: variable_of CO_350:0000011

[Term]
id: CO_350:0000162
name: Groat content (machine dehulled) - percent
namespace: oat_trait
def: "TRAIT: Groat content METHOD: Calculated as the weight of the groat divided by the weight of the whole grain, multiplied by 100. Kernels are typically dehulled using a Codema oat dehuller, which processes a 50 gram sample. SCALE: percent" []
relationship: variable_of CO_350:0000009
relationship: variable_of CO_350:0000010
relationship: variable_of CO_350:0000011

[Term]
id: CO_350:0000163
name: Groat oil content - percent
namespace: oat_trait
def: "TRAIT: The amount of oil in the groat, expressed as a percentage of the groat. METHOD: Computation of the percentage of oil in the groat. SCALE: percent" []
relationship: variable_of CO_350:0000051
relationship: variable_of CO_350:0000052
relationship: variable_of CO_350:0000011

[Term]
id: CO_350:0000164
name: Groat protein content - percent
namespace: oat_trait
def: "TRAIT: The amount of protein in the groat, expressed as a percentage of the groat. METHOD: Computation of the percentage of protein in the groat. SCALE: percent" []
relationship: variable_of CO_350:0000011
relationship: variable_of CO_350:0000055
relationship: variable_of CO_350:0000054

[Term]
id: CO_350:0000165
name: Lodging incidence - percent
namespace: oat_trait
def: "TRAIT: Measure of the percentage of the stems of plants in a plot that have been permanently bent, usually as a result of adverse weather. METHOD: Visual assessement of the percentage of plants that lodged in a plot. SCALE: percent" []
relationship: variable_of CO_350:0000011
relationship: variable_of CO_350:0000016
relationship: variable_of CO_350:0000015

[Term]
id: CO_350:0000166
name: Powdery mildew incidence - percent
namespace: oat_trait
def: "TRAIT: Percentage of plants in a plot showing symptoms of powdery mildew. METHOD: Visual assessment of the percentage of plants in a plot showing symptoms of a specific disease. SCALE: percent" []
relationship: variable_of CO_350:0000011
relationship: variable_of CO_350:0000099
relationship: variable_of CO_350:0000082

[Term]
id: CO_350:0000167
name: Root rot incidence - percent
namespace: oat_trait
def: "TRAIT: Percentage of plants in a plot showing symptoms of root rot. METHOD: Visual assessment of the percentage of plants in a plot showing symptoms of a specific disease. SCALE: percent" []
relationship: variable_of CO_350:0000011
relationship: variable_of CO_350:0000102
relationship: variable_of CO_350:0000082

[Term]
id: CO_350:0000168
name: Smut incidence - percent
namespace: oat_trait
def: "TRAIT: Percentage of plants in a plot showing symptoms of smut. METHOD: Visual assessment of the percentage of plants in a plot showing symptoms of a specific disease. SCALE: percent" []
relationship: variable_of CO_350:0000082
relationship: variable_of CO_350:0000105
relationship: variable_of CO_350:0000011

[Term]
id: CO_350:0000169
name: Stem rust incidence - percent
namespace: oat_trait
def: "TRAIT: Percentage of plants in a plot showing symptoms of stem rust. METHOD: Visual assessment of the percentage of plants in a plot showing symptoms of a specific disease. SCALE: percent" []
relationship: variable_of CO_350:0000082
relationship: variable_of CO_350:0000108
relationship: variable_of CO_350:0000011

[Term]
id: CO_350:0000170
name: Winter survival - percent
namespace: oat_trait
def: "TRAIT: Percentage of plants in a plot sown in fall that are still growing in spring. METHOD: Visual assessement of the percentage of living plants in a plot. SCALE: percent" []
relationship: variable_of CO_350:0000030
relationship: variable_of CO_350:0000031
relationship: variable_of CO_350:0000011

[Term]
id: CO_350:0000174
name: Leaf blotch severity - 0-9 disease severity scale
namespace: oat_trait
def: "TRAIT: Severity of leaf blotch symptoms observed in a plot. METHOD: Visual assessment of the severity of disease symptoms observed in a plot. SCALE: 0-9 disease severity scale" []
relationship: variable_of CO_350:0000085
relationship: variable_of CO_350:0000096
relationship: variable_of CO_350:0000086

[Term]
id: CO_350:0000182
name: Breakage incidence - 1-10 breakage incidence scale
namespace: oat_trait
def: "TRAIT: Proportion of the stems in a plot that are snapped/broken. METHOD: Rating based on the proportion of stems in a plot that are broken/snapped. SCALE: 1-10 breakage incidence scale" []
relationship: variable_of CO_350:0000005
relationship: variable_of CO_350:0000004
relationship: variable_of CO_350:0000003

[Term]
id: CO_350:0000184
name: Groat color - 1-4 groat color scale
namespace: oat_trait
def: "TRAIT: Color of the de-hulled grain: the groat. METHOD: Visual assessement of the color of the groat. SCALE: 1-4 groat color scale (1= light red, 2= light brown, 3= medium brown, 4= dark brown)" []
relationship: variable_of CO_350:0000073
relationship: variable_of CO_350:0000072
relationship: variable_of CO_350:0000074

[Term]
id: CO_350:0000185
name: Agronomic score - 1-5 agronomic score scale
namespace: oat_trait
def: "TRAIT: Rating of overall agronomical attributes and health of oat plants in a plot. METHOD: Scored based on observance of factors limiting yield. SCALE: 1-5 agronomic score scale" []
relationship: variable_of CO_350:0000001
relationship: variable_of CO_350:0000000
relationship: variable_of CO_350:0000002

[Term]
id: CO_350:0000212
name: Relative canopy development - 1-9 relative canopy development scale
namespace: oat_trait
def: "TRAIT: Relative canopy development, each genotype is rated against the earliest genotypes, when those genotypes have a completely closed canopy. METHOD: Visual assessment of the development of the canopy of a plot relative to genotypes with a closed canopy. SCALE: 1-9 relative canopy development scale" []
relationship: variable_of CO_350:0000025
relationship: variable_of CO_350:0000024
relationship: variable_of CO_350:0000026

[Term]
id: CO_350:0000217
name: Snapback - 1-9 snapback scale
namespace: oat_trait
def: "TRAIT: Snapback, or recovery to a vertical position, of the plant after being held at a 45 degree angle. METHOD: Plants are held at a 45 degree angle and released. The snapback, or recovery to vertical position, is rated. SCALE: 1-9 snapback scale" []
relationship: variable_of CO_350:0000027
relationship: variable_of CO_350:0000028
relationship: variable_of CO_350:0000029

[Term]
id: CO_350:0000232
name: Plant height - cm
namespace: oat_trait
def: "TRAIT: Height of plant from ground to top of flag leaf ligule. METHOD: Measurement of the height of the whole plant from the soil surface to the tip of the panicle. SCALE: cm" []
relationship: variable_of CO_350:0000022
relationship: variable_of CO_350:0000021
relationship: variable_of CO_350:0000023

[Term]
id: CO_350:0000251
name: Thousand grain weight - g
namespace: oat_trait
def: "TRAIT: The thousand grain weight. METHOD: Measurement of the weight of 1000 well-developed whole grains. SCALE: g" []
relationship: variable_of CO_350:0000078
relationship: variable_of CO_350:0000079
relationship: variable_of CO_350:0000249

[Term]
id: CO_350:0000258
name: Undehulled seed - g
namespace: oat_trait
def: "TRAIT: Amount of undehulled seed remaining after dehulling. METHOD: Amount of undehulled seed remaining after passing a 50 gram sample through a Codema dehuller, under standard conditions, for 90 seconds. SCALE: g" []
relationship: variable_of CO_350:0000063
relationship: variable_of CO_350:0000064
relationship: variable_of CO_350:0000249

[Term]
id: CO_350:0000259
name: Test weight - g/L
namespace: oat_trait
def: "TRAIT: A measure of the density or weight per unit volume of a grain at a standardized moisture level. SCALE: g/L" []
relationship: variable_of CO_350:0000077
relationship: variable_of CO_350:0000075
relationship: variable_of CO_350:0000076

[Term]
id: CO_350:0000260
name: Grain yield - g/m2
namespace: oat_trait
def: "TRAIT: Total weight of grains harvested per unit area. METHOD: Measurement of the total weight of whole grains harvested per unit area. SCALE: g/m2" []
relationship: variable_of CO_350:0000008
relationship: variable_of CO_350:0000006
relationship: variable_of CO_350:0000007

[Term]
id: CO_350:0000270
name: Heading date - Julian day
namespace: oat_trait
def: "TRAIT: The time when heading occurs. METHOD: Record of the date on which heading occurs. SCALE: Julian day" []
relationship: variable_of CO_350:0000012
relationship: variable_of CO_350:0000013
relationship: variable_of CO_350:0000014

[Term]
id: CO_350:0000271
name: Maturity date - Julian day
namespace: oat_trait
def: "TRAIT: The time when maturity occurs METHOD: Record of the date on which maturity occurs. SCALE: Julian day" []
relationship: variable_of CO_350:0000019
relationship: variable_of CO_350:0000018
relationship: variable_of CO_350:0000014

[Term]
id: CO_350:0000536
name: Grain moisture content - percent
namespace: oat_trait
def: "TRAIT: Moisture content of grain. METHOD: Calculate the mositure content from fresh and dry grain weight. SCALE: percent" []
relationship: variable_of CO_350:0000535
relationship: variable_of CO_350:0000120
relationship: variable_of CO_350:0000011

[Term]
id: CO_350:0000574
name: Lipid content - percent
namespace: oat_trait
def: "TRAIT: The lipid content of the grain. METHOD: Measurement of the percentage of lipid content in grain; prediction obtained using near-infrared spectroscopy (NIR). SCALE: percent" []
relationship: variable_of CO_350:0000011
relationship: variable_of CO_350:0000572
relationship: variable_of CO_350:0000573

[Term]
id: CO_350:0000627
name: Stem rust severity (plant) - percent
namespace: oat_trait
def: "TRAIT: Stem rust severity. METHOD: Observe relative or absolute area of plant tissue affected by Stem rust and record it. Often severity is represented as a proportion or percentage of plant surface affected. SCALE: percent" []
relationship: variable_of CO_350:0000114
relationship: variable_of CO_350:0000626
relationship: variable_of CO_350:0000011

[Term]
id: CO_350:0000646
name: Deoxynivalenol concentration - ppm
namespace: oat_trait
def: "TRAIT: Amount of the mycotoxin deoxynivalenol found in the grain after an infection by Fusarium sp. METHOD: Computation of the deoxynivalenol content SCALE: ppm" []
relationship: variable_of CO_350:0000047
relationship: variable_of CO_350:0000046
relationship: variable_of CO_350:0000045

[Term]
id: CO_350:0000671
name: Avenanthramide content - ug/g
namespace: oat_trait
def: "TRAIT: Avenanthramide content METHOD: Direct measurement of the total avenanthramide content SCALE: ug/g" []
relationship: variable_of CO_350:0000034
relationship: variable_of CO_350:0000033
relationship: variable_of CO_350:0000035

[Term]
id: CO_350:0005001
name: Freeze damage severity - 0-9 Rating
namespace: oat_trait
def: "TRAIT: Severity of the symptoms of freeze damage observed in a plot METHOD: Estimation of the freeze damage severity using a 0-9 scale: 0= no freeze damage, 9= severe freeze damage. SCALE: 0-9 rating scale" []
relationship: variable_of CO_350:0005901
relationship: variable_of CO_350:0005601
relationship: variable_of CO_350:0005401

[Term]
id: CO_350:0005002
name: Storm damage severity - 1-5 Rating
namespace: oat_trait
def: "TRAIT: Severity of the damage inflicted by stormy weather METHOD: Estimation of the storm damage severity using a 1-5 scale: 1= no damage, 5= total damage and loss of plot. SCALE: 1-5 rating scale" []
relationship: variable_of CO_350:0005602
relationship: variable_of CO_350:0005402
relationship: variable_of CO_350:0005902

[Term]
id: CO_350:0005003
name: Winter stress severity - 0-9 Rating
namespace: oat_trait
def: "TRAIT: Mid-winter rating of the severity of the symptoms of winter stress observed in a plot METHOD: Estimation of the winter stress severity using a 0-9 scale: 0= no signs of winter stress, 9= severe leaf damage or leaves that are purple in color.	 SCALE: 0-9 rating scale" []
relationship: variable_of CO_350:0005901
relationship: variable_of CO_350:0005403
relationship: variable_of CO_350:0005603

[Term]
id: CO_350:0005004
name: Emergence - %
namespace: oat_trait
def: "TRAIT: Percentage of plants in a plot that have emerged METHOD: Measurement of the percentage of plants in a plot that have emerged SCALE: percent" []
relationship: variable_of CO_350:0005604
relationship: variable_of CO_350:0005404
relationship: variable_of CO_350:0000011

[Term]
id: CO_350:0005005
name: Forage rating - 0-9 Rating
namespace: oat_trait
def: "TRAIT: Yield potential in spring METHOD: Estimation of the forage rating using a 0-9 scale: 0= low, 9= high SCALE: 0-9 rating scale" []
relationship: variable_of CO_350:0005901
relationship: variable_of CO_350:0005405
relationship: variable_of CO_350:0005605

[Term]
id: CO_350:0005006
name: Groat content (hand dehulled) - %
namespace: oat_trait
def: "TRAIT: Groat content METHOD: Calculated as the total groat weight divided by the initial kernel weight before dehulling, multiplied by 100. Kernels are dehulled by hand and sample sizes are smaller than for machine dehulling, for example two grams. SCALE: percent" []
relationship: variable_of CO_350:0000011
relationship: variable_of CO_350:0000009
relationship: variable_of CO_350:0005606

[Term]
id: CO_350:0005007
name: Lodging severity - 0-9 Rating
namespace: oat_trait
def: "TRAIT: Severity of lodging symptoms observed in a plot: lodged plants do not stand erect. METHOD: Visual assessment of the severity of lodging observed in a plot. SCALE: 0-9 rating scale" []
relationship: variable_of CO_350:0005901
relationship: variable_of CO_350:0000118
relationship: variable_of CO_350:0000117

[Term]
id: CO_350:0005008
name: Phenotype score - 0-9 Rating
namespace: oat_trait
def: "TRAIT: Relative rating of visual appeal that takes in to account plant vigor, diseases, etc. METHOD: Visual assessment of the phenotype score using a 0-9 scale: 0= perfect, 1= excellent, 4= good, 5= borderline, 6= poor, 9= unadapted SCALE: 0-9 rating scale" []
relationship: variable_of CO_350:0005901
relationship: variable_of CO_350:0005406
relationship: variable_of CO_350:0005607

[Term]
id: CO_350:0005009
name: Silage yield (65% moisture) - t/ac
namespace: oat_trait
def: "TRAIT: Total weight of silage per unit area METHOD: Silage yield at 65% moisture content SCALE: t/ac" []
relationship: variable_of CO_350:0005903
relationship: variable_of CO_350:0005407
relationship: variable_of CO_350:0005608

[Term]
id: CO_350:0005010
name: Silage yield (dry matter) - t/ac
namespace: oat_trait
def: "TRAIT: Total weight of silage per unit area METHOD: Yield of dry matter for use as silage SCALE: t/ac" []
relationship: variable_of CO_350:0005609
relationship: variable_of CO_350:0005407
relationship: variable_of CO_350:0005903

[Term]
id: CO_350:0005011
name: Barley yellow dwarf virus severity - 0-9 Rating
namespace: oat_trait
def: "TRAIT: Severity of barley yellow dwarf virus symptoms observed in a plot. METHOD: Estimation of the severity of barley yellow dwarf virus symptoms observed in a plot; plots rated 0 exhibit essentially no chlorosis, no stunted tillers, and no blasting, plots rated 9 do not head and are very severely stunted. SCALE: 0-9 rating scale" []
relationship: variable_of CO_350:0005901
relationship: variable_of CO_350:0000084
relationship: variable_of CO_350:0005610

[Term]
id: CO_350:0005012
name: Bird damage severity - 0-9 Rating
namespace: oat_trait
def: "TRAIT: Severity of the symptoms of bird damage observed in a plot METHOD: Estimation of the severity of the symptoms of bird damage on a 0-9 scale: 0= no bird damage, 9= severe bird damage SCALE: 0-9 rating scale" []
relationship: variable_of CO_350:0005611
relationship: variable_of CO_350:0005408
relationship: variable_of CO_350:0005901

[Term]
id: CO_350:0005013
name: Cereal leaf beetle damage severity - 0-3 Rating
namespace: oat_trait
def: "TRAIT: Severity of larval feeding damage caused by cereal leaf beetle (Oulema malanopus). METHOD: Estimation of the severity of cereal leaf beetle damage on a 0-3 scale: 0= no larval feeding, 1= 1-15% foliage eaten, 2= 15-40% foliage eaten, 3= over 40% foliage eaten SCALE: 1-3 rating scale" []
relationship: variable_of CO_350:0005904
relationship: variable_of CO_350:0005612
relationship: variable_of CO_350:0005409

[Term]
id: CO_350:0005014
name: Crown rust infection response - 0-1 Disease Infection Response Rating
namespace: oat_trait
def: "TRAIT: A qualitative analysis of the type of crown rust symptoms that are exhibited. METHOD: Estimation of the crown rust infection response. 	A qualitative analysis of the type of crown rust (Puccinia coronata f. sp. avenae) symptoms that are exhibited. Infection responses are limited to: Resistant (R): chlorotic fleck reaction with no sporulation; Moderately resistant (MR): Very small, non- or low-sporulating pustule surrounded by chlorosis; Moderately susceptible (MS): moderate to large pustule surrounded by extensive chlorosis, and; Susceptible (S): large pustule with little or no chlorosis. The following numerical scale has been used to quantify conventional notations of infection type: R= 0.2, R-MR= 0.3, MR= 0.4, R-MS= 0.45, R-S= 0.5, MR-MS= 0.6, MR-S= 0.7, MS= 0.8, MS-S= 0.9, S=1. Crown rust infection response is typically recorded in conjunction with crown rust severity. SCALE: Disease Infection Response Rating (0-1) (0.2= R, 0.3= R-MR, 0.4= MR, 0.45= R-MS, 0.5= R-S, 0.6= MR-MS, 0.7= MR-S, 0.8= MS, 0.9= MS-S, 1.0= S)" []
relationship: variable_of CO_350:0000087
relationship: variable_of CO_350:0005613
relationship: variable_of CO_350:0005905

[Term]
id: CO_350:0005015
name: Crown rust infection type - BQBC - 0-4 Murphy Infection Type Rating
namespace: oat_trait
def: "TRAIT: A qualitative analysis of the type of crown rust symptoms that are exhibited. METHOD: A qualitative analysis of the type of disease symptoms exhibited by seedlings inoculated with crown rust (Puccinia coronata f. sp. avenae) race BQBC during greenhouse trials. Ratings made using the scale from Murphy (1935); immune/nearly immune= 0, highly resistant= 1, moderately resistant= 2, moderately susceptible= 3, and completely susceptible= 4. SCALE: Murphy Infection Type Rating (0-4) (0= immune/nearly immune, 1= highly resistant, 2= moderately resistant, 3= moderately susceptible, 4= completely susceptible)" []
relationship: variable_of CO_350:0005906
relationship: variable_of CO_350:0000087
relationship: variable_of CO_350:0005614

[Term]
id: CO_350:0005016
name: Crown rust infection type - BRBG-94 - 0-4 Murphy Infection Type Rating
namespace: oat_trait
def: "TRAIT: A qualitative analysis of the type of crown rust symptoms that are exhibited. METHOD: A qualitative analysis of the type of disease symptoms exhibited by seedlings inoculated with crown rust (Puccinia coronata f. sp. avenae) race BRBG-94 during greenhouse trials. Ratings made using the scale from Murphy (1935); immune/nearly immune= 0, highly resistant= 1, moderately resistant= 2, moderately susceptible= 3, and completely susceptible= 4. SCALE: Murphy Infection Type Rating (0-4) (0= immune/nearly immune, 1= highly resistant, 2= moderately resistant, 3= moderately susceptible, 4= completely susceptible)" []
relationship: variable_of CO_350:0000087
relationship: variable_of CO_350:0005615
relationship: variable_of CO_350:0005906

[Term]
id: CO_350:0005017
name: Crown rust infection type - Composite/Unknown - 0-4 Murphy Infection Type Rating
namespace: oat_trait
def: "TRAIT: A qualitative analysis of the type of crown rust symptoms that are exhibited. METHOD: A qualitative analysis of the type of disease symptoms exhibited by seedlings inoculated with crown rust (Puccinia coronata f. sp. avenae) composite race / unknown race during greenhouse trials. Ratings made using the scale from Murphy (1935); immune/nearly immune= 0, highly resistant= 1, moderately resistant= 2, moderately susceptible= 3, and completely susceptible= 4. SCALE: Murphy Infection Type Rating (0-4) (0= immune/nearly immune, 1= highly resistant, 2= moderately resistant, 3= moderately susceptible, 4= completely susceptible)" []
relationship: variable_of CO_350:0005906
relationship: variable_of CO_350:0005616
relationship: variable_of CO_350:0000087

[Term]
id: CO_350:0005018
name: Crown rust infection type - DQBB - 0-4 Murphy Infection Type Rating
namespace: oat_trait
def: "TRAIT: A qualitative analysis of the type of crown rust symptoms that are exhibited. METHOD: A qualitative analysis of the type of disease symptoms exhibited by seedlings inoculated with crown rust (Puccinia coronata f. sp. avenae) race DQBB during greenhouse trials. Ratings made using the scale from Murphy (1935); immune/nearly immune= 0, highly resistant= 1, moderately resistant= 2, moderately susceptible= 3, and completely susceptible= 4. SCALE: Murphy Infection Type Rating (0-4) (0= immune/nearly immune, 1= highly resistant, 2= moderately resistant, 3= moderately susceptible, 4= completely susceptible)" []
relationship: variable_of CO_350:0005617
relationship: variable_of CO_350:0000087
relationship: variable_of CO_350:0005906

[Term]
id: CO_350:0005019
name: Crown rust infection type - DQBG - 0-4 Murphy Infection Type Rating
namespace: oat_trait
def: "TRAIT: A qualitative analysis of the type of crown rust symptoms that are exhibited. METHOD: A qualitative analysis of the type of disease symptoms exhibited by seedlings inoculated with crown rust (Puccinia coronata f. sp. avenae) race DQBG during greenhouse trials. Ratings made using the scale from Murphy (1935); immune/nearly immune= 0, highly resistant= 1, moderately resistant= 2, moderately susceptible= 3, and completely susceptible= 4. SCALE: Murphy Infection Type Rating (0-4) (0= immune/nearly immune, 1= highly resistant, 2= moderately resistant, 3= moderately susceptible, 4= completely susceptible)" []
relationship: variable_of CO_350:0005906
relationship: variable_of CO_350:0000087
relationship: variable_of CO_350:0005618

[Term]
id: CO_350:0005020
name: Crown rust infection type - DSGB - 0-4 Murphy Infection Type Rating
namespace: oat_trait
def: "TRAIT: A qualitative analysis of the type of crown rust symptoms that are exhibited. METHOD: A qualitative analysis of the type of disease symptoms exhibited by seedlings inoculated with crown rust (Puccinia coronata f. sp. avenae) race DSGB during greenhouse trials. Ratings made using the scale from Murphy (1935); immune/nearly immune= 0, highly resistant= 1, moderately resistant= 2, moderately susceptible= 3, and completely susceptible= 4. SCALE: Murphy Infection Type Rating (0-4) (0= immune/nearly immune, 1= highly resistant, 2= moderately resistant, 3= moderately susceptible, 4= completely susceptible)" []
relationship: variable_of CO_350:0000087
relationship: variable_of CO_350:0005619
relationship: variable_of CO_350:0005906

[Term]
id: CO_350:0005021
name: Crown rust infection type - LQCB-91 - 0-4 Murphy Infection Type Rating
namespace: oat_trait
def: "TRAIT: A qualitative analysis of the type of crown rust symptoms that are exhibited. METHOD: A qualitative analysis of the type of disease symptoms exhibited by seedlings inoculated with crown rust (Puccinia coronata f. sp. avenae) race LQCB-91 during greenhouse trials. Ratings made using the scale from Murphy (1935); immune/nearly immune= 0, highly resistant= 1, moderately resistant= 2, moderately susceptible= 3, and completely susceptible= 4. SCALE: Murphy Infection Type Rating (0-4) (0= immune/nearly immune, 1= highly resistant, 2= moderately resistant, 3= moderately susceptible, 4= completely susceptible)" []
relationship: variable_of CO_350:0005906
relationship: variable_of CO_350:0005620
relationship: variable_of CO_350:0000087

[Term]
id: CO_350:0005022
name: Crown rust infection type - LRBG - 0-4 Murphy Infection Type Rating
namespace: oat_trait
def: "TRAIT: A qualitative analysis of the type of crown rust symptoms that are exhibited. METHOD: A qualitative analysis of the type of disease symptoms exhibited by seedlings inoculated with crown rust (Puccinia coronata f. sp. avenae) race LRBG during greenhouse trials. Ratings made using the scale from Murphy (1935); immune/nearly immune= 0, highly resistant= 1, moderately resistant= 2, moderately susceptible= 3, and completely susceptible= 4. SCALE: Murphy Infection Type Rating (0-4) (0= immune/nearly immune, 1= highly resistant, 2= moderately resistant, 3= moderately susceptible, 4= completely susceptible)" []
relationship: variable_of CO_350:0005906
relationship: variable_of CO_350:0000087
relationship: variable_of CO_350:0005621

[Term]
id: CO_350:0005023
name: Crown rust infection type - MHBB - 0-4 Murphy Infection Type Rating
namespace: oat_trait
def: "TRAIT: A qualitative analysis of the type of crown rust symptoms that are exhibited. METHOD: A qualitative analysis of the type of disease symptoms exhibited by seedlings inoculated with crown rust (Puccinia coronata f. sp. avenae) race MHBB during greenhouse trials. Ratings made using the scale from Murphy (1935); immune/nearly immune= 0, highly resistant= 1, moderately resistant= 2, moderately susceptible= 3, and completely susceptible= 4. SCALE: Murphy Infection Type Rating (0-4) (0= immune/nearly immune, 1= highly resistant, 2= moderately resistant, 3= moderately susceptible, 4= completely susceptible)" []
relationship: variable_of CO_350:0005906
relationship: variable_of CO_350:0000087
relationship: variable_of CO_350:0005622

[Term]
id: CO_350:0005024
name: Crown rust infection type - NBFB - 0-4 Murphy Infection Type Rating
namespace: oat_trait
def: "TRAIT: A qualitative analysis of the type of crown rust symptoms that are exhibited. METHOD: A qualitative analysis of the type of disease symptoms exhibited by seedlings inoculated with crown rust (Puccinia coronata f. sp. avenae) race NBFB during greenhouse trials. Ratings made using the scale from Murphy (1935); immune/nearly immune= 0, highly resistant= 1, moderately resistant= 2, moderately susceptible= 3, and completely susceptible= 4. SCALE: Murphy Infection Type Rating (0-4) (0= immune/nearly immune, 1= highly resistant, 2= moderately resistant, 3= moderately susceptible, 4= completely susceptible)" []
relationship: variable_of CO_350:0005906
relationship: variable_of CO_350:0005623
relationship: variable_of CO_350:0000087

[Term]
id: CO_350:0005025
name: Crown rust infection type - NGCC-94 - 0-4 Murphy Infection Type Rating
namespace: oat_trait
def: "TRAIT: A qualitative analysis of the type of crown rust symptoms that are exhibited. METHOD: A qualitative analysis of the type of disease symptoms exhibited by seedlings inoculated with crown rust (Puccinia coronata f. sp. avenae) race NGCC-94 during greenhouse trials. Ratings made using the scale from Murphy (1935); immune/nearly immune= 0, highly resistant= 1, moderately resistant= 2, moderately susceptible= 3, and completely susceptible= 4. SCALE: Murphy Infection Type Rating (0-4) (0= immune/nearly immune, 1= highly resistant, 2= moderately resistant, 3= moderately susceptible, 4= completely susceptible)" []
relationship: variable_of CO_350:0005906
relationship: variable_of CO_350:0000087
relationship: variable_of CO_350:0005624

[Term]
id: CO_350:0005026
name: Crown rust infection type - NQBB - 0-4 Murphy Infection Type Rating
namespace: oat_trait
def: "TRAIT: A qualitative analysis of the type of crown rust symptoms that are exhibited. METHOD: A qualitative analysis of the type of disease symptoms exhibited by seedlings inoculated with crown rust (Puccinia coronata f. sp. avenae) race NQBB during greenhouse trials. Ratings made using the scale from Murphy (1935); immune/nearly immune= 0, highly resistant= 1, moderately resistant= 2, moderately susceptible= 3, and completely susceptible= 4. SCALE: Murphy Infection Type Rating (0-4) (0= immune/nearly immune, 1= highly resistant, 2= moderately resistant, 3= moderately susceptible, 4= completely susceptible)" []
relationship: variable_of CO_350:0005625
relationship: variable_of CO_350:0000087
relationship: variable_of CO_350:0005906

[Term]
id: CO_350:0005027
name: Crown rust infection type - NTGG - 0-4 Murphy Infection Type Rating
namespace: oat_trait
def: "TRAIT: A qualitative analysis of the type of crown rust symptoms that are exhibited. METHOD: A qualitative analysis of the type of disease symptoms exhibited by seedlings inoculated with crown rust (Puccinia coronata f. sp. avenae) race NTGG during greenhouse trials. Ratings made using the scale from Murphy (1935); immune/nearly immune= 0, highly resistant= 1, moderately resistant= 2, moderately susceptible= 3, and completely susceptible= 4. SCALE: Murphy Infection Type Rating (0-4) (0= immune/nearly immune, 1= highly resistant, 2= moderately resistant, 3= moderately susceptible, 4= completely susceptible)" []
relationship: variable_of CO_350:0000087
relationship: variable_of CO_350:0005626
relationship: variable_of CO_350:0005906

[Term]
id: CO_350:0005028
name: Crown rust infection type - SJGL - 0-4 Murphy Infection Type Rating
namespace: oat_trait
def: "TRAIT: A qualitative analysis of the type of crown rust symptoms that are exhibited. METHOD: A qualitative analysis of the type of disease symptoms exhibited by seedlings inoculated with crown rust (Puccinia coronata f. sp. avenae) race SJGL during greenhouse trials. Ratings made using the scale from Murphy (1935); immune/nearly immune= 0, highly resistant= 1, moderately resistant= 2, moderately susceptible= 3, and completely susceptible= 4. SCALE: Murphy Infection Type Rating (0-4) (0= immune/nearly immune, 1= highly resistant, 2= moderately resistant, 3= moderately susceptible, 4= completely susceptible)" []
relationship: variable_of CO_350:0005906
relationship: variable_of CO_350:0000087
relationship: variable_of CO_350:0005627

[Term]
id: CO_350:0005029
name: Crown rust severity (flag leaf) - percent
namespace: oat_trait
def: "TRAIT: Crown rust severity. METHOD: Estimation of the percentage of the area of the flag leaf occupied by crown rust (Puccinia coronata f. sp. avenae) pustules or necrosis, following the modified Cobb scale (Peterson et al. 1948) and recorded in conjunction with crown rust infection response. Common intervals: trace (0.1 in T3), 5, 10, 20, 40, 60, and 100 percent infection. SCALE: percent" []
relationship: variable_of CO_350:0000011
relationship: variable_of CO_350:0005628
relationship: variable_of CO_350:0000090

[Term]
id: CO_350:0005030
name: Crown rust severity (plot) - 0-9 Rating
namespace: oat_trait
def: "TRAIT: Crown rust severity. METHOD: Estimation of the severity of crown rust (Puccinia coronata f. sp. avenae) symptoms observed in a plot; plots rated 0 exhibit no symptoms, plots rated 9 show severe symptoms. SCALE: 0-9 rating scale" []
relationship: variable_of CO_350:0005629
relationship: variable_of CO_350:0000090
relationship: variable_of CO_350:0005901

[Term]
id: CO_350:0005031
name: Crown rust severity (whole plant) - 9-1 Rating
namespace: oat_trait
def: "TRAIT: Crown rust severity. METHOD: Estimation of the severity of crown rust (Puccinia coronata f. sp. avenae) symptoms. Ratings based on the percent infection of the whole plant; 79-100%= 1, 90-97%= 2, 75-90%= 3, 60-75%= 4, 40-60%= 5, 25-40%= 6, 10-25%= 7, 3-10%= 8, 0-3%= 9. SCALE: 9-1 rating scale (9= low, 1= high)" []
relationship: variable_of CO_350:0005630
relationship: variable_of CO_350:0000090
relationship: variable_of CO_350:0005907

[Term]
id: CO_350:0005032
name: Downy mildew severity - 0-9 Rating
namespace: oat_trait
def: "TRAIT: Downy mildew severity. METHOD: Estimation of the severity of downy mildew (Sclerophthora macrospora) symptoms observed in a plot; plots rated 0 exhibit no symptoms, plots rated 9 show severe symptoms.	 SCALE: 0-9 rating scale" []
relationship: variable_of CO_350:0005631
relationship: variable_of CO_350:0000523
relationship: variable_of CO_350:0005901

[Term]
id: CO_350:0005033
name: Fusarium head blight incidence - 0-4 Rating
namespace: oat_trait
def: "TRAIT: Percentage of plants in a plot showing Fusarium head blight symptoms. METHOD: Estimation of the incidence of Fusarium head blight (Fusarium spp.; FHB) symptoms observed in a plot; plots rated 0 exhibit no FHB symptoms, plots rated 1 contain a few blighted spikelets, while a rating of 4 indicates that the whole plot is blighted. SCALE: 0-4 rating scale" []
relationship: variable_of CO_350:0005908
relationship: variable_of CO_350:0005632
relationship: variable_of CO_350:0000093

[Term]
id: CO_350:0005034
name: Stagonospora severity - 0-9 Rating
namespace: oat_trait
def: "TRAIT: Severity of Stagonospora avenae f. sp. avenaria symptoms. Stagonospora causes leaf blotch and black stem of oat. METHOD: Estimation of the severity Stagonospora avenae f. sp. avenaria symptoms in a plot using a 0-9 scale: 0= no symptoms, 9= high symptoms. SCALE: 0-9 rating scale" []
relationship: variable_of CO_350:0005633
relationship: variable_of CO_350:0005410
relationship: variable_of CO_350:0005901

[Term]
id: CO_350:0005035
name: Stem rust infection response - 0-1 Disease Infection Response Rating
namespace: oat_trait
def: "TRAIT: A qualitative analysis of the type of stem rust symptoms that are exhibited. METHOD: Estimation of the stem rust infection response. A qualitative analysis of the type of stem rust (Puccinia graminis f. sp. avenae) symptoms that are exhibited. Infection responses are limited to: Resistant (R): chlorotic fleck reaction with no sporulation; Moderately resistant (MR): Very small, non- or low-sporulating pustule surrounded by chlorosis; Moderately susceptible (MS): moderate to large pustule surrounded by extensive chlorosis, and; Susceptible (S): large pustule with little or no chlorosis. The following numerical scale has been used to quantify conventional notations of infection type: R= 0.2, R-MR= 0.3, MR= 0.4, R-MS= 0.45, R-S= 0.5, MR-MS= 0.6, MR-S= 0.7, MS= 0.8, MS-S= 0.9, S=1. Stem rust infection response is typically recorded in conjunction with stem rust severity. SCALE: Disease Infection Response Rating (0-1) (0.2= R, 0.3= R-MR, 0.4= MR, 0.45= R-MS, 0.5= R-S, 0.6= MR-MS, 0.7= MR-S, 0.8= MS, 0.9= MS-S, 1.0= S)" []
relationship: variable_of CO_350:0005905
relationship: variable_of CO_350:0000111
relationship: variable_of CO_350:0005634

[Term]
id: CO_350:0005036
name: Stem rust infection type - Composite - 0-4 Murphy Infection Type Rating
namespace: oat_trait
def: "TRAIT: A qualitative analysis of the type of stem rust symptoms that are exhibited. METHOD: A qualitative analysis of the type of disease symptoms exhibited by seedlings inoculated with a composite collection or unknown race of stem rust (Puccinia graminis f. sp. avenae) during greenhouse trials. Ratings made using the scale from Stakman et al. (1962); immune= 0, very resistant= 1, moderately resistant= 2, moderately susceptible= 3, and very susceptible= 4. SCALE: Murphy Infection Type Rating (0-4) (0= immune/nearly immune, 1= highly resistant, 2= moderately resistant, 3= moderately susceptible, 4= completely susceptible)" []
relationship: variable_of CO_350:0005906
relationship: variable_of CO_350:0000111
relationship: variable_of CO_350:0005635

[Term]
id: CO_350:0005037
name: Stem rust infection type - NA1 - 0-4 Murphy Infection Type Rating
namespace: oat_trait
def: "TRAIT: A qualitative analysis of the type of stem rust symptoms that are exhibited. METHOD: A qualitative analysis of the type of disease symptoms exhibited by seedlings inoculated with stem rust (Puccinia graminis f. sp. avenae) race NA1 during greenhouse trials. Ratings made using the scale from Stakman et al. (1962); immune= 0, very resistant= 1, moderately resistant= 2, moderately susceptible= 3, and very susceptible= 4.  SCALE: Murphy Infection Type Rating (0-4) (0= immune/nearly immune, 1= highly resistant, 2= moderately resistant, 3= moderately susceptible, 4= completely susceptible)" []
relationship: variable_of CO_350:0005636
relationship: variable_of CO_350:0000111
relationship: variable_of CO_350:0005906

[Term]
id: CO_350:0005038
name: Stem rust infection type - NA16 - 0-4 Murphy Infection Type Rating
namespace: oat_trait
def: "TRAIT: A qualitative analysis of the type of stem rust symptoms that are exhibited. METHOD: A qualitative analysis of the type of disease symptoms exhibited by seedlings inoculated with stem rust (Puccinia graminis f. sp. avenae) race NA16 during greenhouse trials. Ratings made using the scale from Stakman et al. (1962); immune= 0, very resistant= 1, moderately resistant= 2, moderately susceptible= 3, and very susceptible= 4.  SCALE: Murphy Infection Type Rating (0-4) (0= immune/nearly immune, 1= highly resistant, 2= moderately resistant, 3= moderately susceptible, 4= completely susceptible)" []
relationship: variable_of CO_350:0000111
relationship: variable_of CO_350:0005637
relationship: variable_of CO_350:0005906

[Term]
id: CO_350:0005039
name: Stem rust infection type - NA25 - 0-4 Murphy Infection Type Rating
namespace: oat_trait
def: "TRAIT: A qualitative analysis of the type of stem rust symptoms that are exhibited. METHOD: A qualitative analysis of the type of disease symptoms exhibited by seedlings inoculated with stem rust (Puccinia graminis f. sp. avenae) race NA25 during greenhouse trials. Ratings made using the scale from Stakman et al. (1962); immune= 0, very resistant= 1, moderately resistant= 2, moderately susceptible= 3, and very susceptible= 4.  SCALE: Murphy Infection Type Rating (0-4) (0= immune/nearly immune, 1= highly resistant, 2= moderately resistant, 3= moderately susceptible, 4= completely susceptible)" []
relationship: variable_of CO_350:0005906
relationship: variable_of CO_350:0005638
relationship: variable_of CO_350:0000111

[Term]
id: CO_350:0005040
name: Stem rust infection type - NA27 - 0-4 Murphy Infection Type Rating
namespace: oat_trait
def: "TRAIT: A qualitative analysis of the type of stem rust symptoms that are exhibited. METHOD: A qualitative analysis of the type of disease symptoms exhibited by seedlings inoculated with stem rust (Puccinia graminis f. sp. avenae) race NA27 during greenhouse trials. Ratings made using the scale from Stakman et al. (1962); immune= 0, very resistant= 1, moderately resistant= 2, moderately susceptible= 3, and very susceptible= 4.  SCALE: Murphy Infection Type Rating (0-4) (0= immune/nearly immune, 1= highly resistant, 2= moderately resistant, 3= moderately susceptible, 4= completely susceptible)" []
relationship: variable_of CO_350:0005906
relationship: variable_of CO_350:0000111
relationship: variable_of CO_350:0005639

[Term]
id: CO_350:0005041
name: Stem rust infection type - NA28 - 0-4 Murphy Infection Type Rating
namespace: oat_trait
def: "TRAIT: A qualitative analysis of the type of stem rust symptoms that are exhibited. METHOD: A qualitative analysis of the type of disease symptoms exhibited by seedlings inoculated with stem rust (Puccinia graminis f. sp. avenae) race NA28 during greenhouse trials. Ratings made using the scale from Stakman et al. (1962); immune= 0, very resistant= 1, moderately resistant= 2, moderately susceptible= 3, and very susceptible= 4.  SCALE: Murphy Infection Type Rating (0-4) (0= immune/nearly immune, 1= highly resistant, 2= moderately resistant, 3= moderately susceptible, 4= completely susceptible)" []
relationship: variable_of CO_350:0005640
relationship: variable_of CO_350:0000111
relationship: variable_of CO_350:0005906

[Term]
id: CO_350:0005042
name: Stem rust infection type - NA29 - 0-4 Murphy Infection Type Rating
namespace: oat_trait
def: "TRAIT: A qualitative analysis of the type of stem rust symptoms that are exhibited. METHOD: A qualitative analysis of the type of disease symptoms exhibited by seedlings inoculated with stem rust (Puccinia graminis f. sp. avenae) race NA29 during greenhouse trials. Ratings made using the scale from Stakman et al. (1962); immune= 0, very resistant= 1, moderately resistant= 2, moderately susceptible= 3, and very susceptible= 4.  SCALE: Murphy Infection Type Rating (0-4) (0= immune/nearly immune, 1= highly resistant, 2= moderately resistant, 3= moderately susceptible, 4= completely susceptible)" []
relationship: variable_of CO_350:0005906
relationship: variable_of CO_350:0000111
relationship: variable_of CO_350:0005641

[Term]
id: CO_350:0005043
name: Stem rust infection type - NA55 - 0-4 Murphy Infection Type Rating
namespace: oat_trait
def: "TRAIT: A qualitative analysis of the type of stem rust symptoms that are exhibited. METHOD: A qualitative analysis of the type of disease symptoms exhibited by seedlings inoculated with stem rust (Puccinia graminis f. sp. avenae) race NA55 during greenhouse trials. Ratings made using the scale from Stakman et al. (1962); immune= 0, very resistant= 1, moderately resistant= 2, moderately susceptible= 3, and very susceptible= 4.  SCALE: Murphy Infection Type Rating (0-4) (0= immune/nearly immune, 1= highly resistant, 2= moderately resistant, 3= moderately susceptible, 4= completely susceptible)" []
relationship: variable_of CO_350:0005906
relationship: variable_of CO_350:0005642
relationship: variable_of CO_350:0000111

[Term]
id: CO_350:0005044
name: Stem rust infection type - NA67 - 0-4 Murphy Infection Type Rating
namespace: oat_trait
def: "TRAIT: A qualitative analysis of the type of stem rust symptoms that are exhibited. METHOD: A qualitative analysis of the type of disease symptoms exhibited by seedlings inoculated with stem rust (Puccinia graminis f. sp. avenae) race NA67 during greenhouse trials. Ratings made using the scale from Stakman et al. (1962); immune= 0, very resistant= 1, moderately resistant= 2, moderately susceptible= 3, and very susceptible= 4.  SCALE: Murphy Infection Type Rating (0-4) (0= immune/nearly immune, 1= highly resistant, 2= moderately resistant, 3= moderately susceptible, 4= completely susceptible)" []
relationship: variable_of CO_350:0005906
relationship: variable_of CO_350:0005643
relationship: variable_of CO_350:0000111

[Term]
id: CO_350:0005045
name: Stem rust infection type - NA8 - 0-4 Murphy Infection Type Rating
namespace: oat_trait
def: "TRAIT: A qualitative analysis of the type of stem rust symptoms that are exhibited. METHOD: A qualitative analysis of the type of disease symptoms exhibited by seedlings inoculated with stem rust (Puccinia graminis f. sp. avenae) race NA8 during greenhouse trials. Ratings made using the scale from Stakman et al. (1962); immune= 0, very resistant= 1, moderately resistant= 2, moderately susceptible= 3, and very susceptible= 4.  SCALE: Murphy Infection Type Rating (0-4) (0= immune/nearly immune, 1= highly resistant, 2= moderately resistant, 3= moderately susceptible, 4= completely susceptible)" []
relationship: variable_of CO_350:0000111
relationship: variable_of CO_350:0005644
relationship: variable_of CO_350:0005906

[Term]
id: CO_350:0005046
name: Stem rust severity (plot) - 0-9 Rating
namespace: oat_trait
def: "TRAIT: Stem rust severity. METHOD: Estimation of the severity of stem rust (Puccinia graminis f. sp. avenae) symptoms observed in a plot; plots rated 0 exhibit no symptoms, plots rated 9 show severe symptoms. SCALE: 0-9 rating scale" []
relationship: variable_of CO_350:0000114
relationship: variable_of CO_350:0005645
relationship: variable_of CO_350:0005901

[Term]
id: CO_350:0005047
name: GC-MS - intensity
namespace: oat_trait
def: "TRAIT: Gas chromatography mass spectrometry METHOD: Direct measurement of a gas chromatography mass spectrum SCALE: mass spectrometry intensity" []
relationship: variable_of CO_350:0005909
relationship: variable_of CO_350:0005646
relationship: variable_of CO_350:0005411

[Term]
id: CO_350:0005048
name: LC-MS - intensity
namespace: oat_trait
def: "TRAIT: Liquid chromatography mass spectrometry METHOD: Direct measurement of a liquid chromatography mass spectrum SCALE: mass spectrometry intensity" []
relationship: variable_of CO_350:0005909
relationship: variable_of CO_350:0005647
relationship: variable_of CO_350:0005412

[Term]
id: CO_350:0005049
name: Grain plumpness - 5.0/64 plump - %
namespace: oat_trait
def: "TRAIT: The amount of a grain sample that does not pass through the holes of a sieve of defined size, expressed as a percentage weight of the entire sample. METHOD: Measurement of the percentage of grain that did not pass through a 5.0/64" sieve. SCALE: percent" []
relationship: variable_of CO_350:0000011
relationship: variable_of CO_350:0005648
relationship: variable_of CO_350:0000066

[Term]
id: CO_350:0005050
name: Grain plumpness - 5.0/64 thin - %
namespace: oat_trait
def: "TRAIT: The amount of a grain sample that does not pass through the holes of a sieve of defined size, expressed as a percentage weight of the entire sample. METHOD: Measurement of the percentage of grain that passed through a 5.0/64" sieve. SCALE: percent" []
relationship: variable_of CO_350:0005649
relationship: variable_of CO_350:0000066
relationship: variable_of CO_350:0000011

[Term]
id: CO_350:0005051
name: Grain plumpness - 5.5/64 plump - %
namespace: oat_trait
def: "TRAIT: The amount of a grain sample that does not pass through the holes of a sieve of defined size, expressed as a percentage weight of the entire sample. METHOD: Measurement of the percentage of grain that did not pass through a 5.5/64" sieve. SCALE: percent" []
relationship: variable_of CO_350:0000011
relationship: variable_of CO_350:0005650
relationship: variable_of CO_350:0000066

[Term]
id: CO_350:0005052
name: Growth habit - 0-9 Rating
namespace: oat_trait
def: "TRAIT: Growth habit rating ranging from very upright spring type to very prostrate winter type METHOD: A visual assessment of the growth habit:  very upright spring type= 0, very prostrate winter type= 9. SCALE: 0-9 rating scale" []
relationship: variable_of CO_350:0005651
relationship: variable_of CO_350:0005413
relationship: variable_of CO_350:0005901

[Term]
id: CO_350:0005053
name: Hull color - 1-10 grain color scale
namespace: oat_trait
def: "TRAIT: Hull color METHOD: A visual assessment of the hull color using a 1-10 rating: white= 1, cream= 2, light tan= 3, yellow= 6, black= 10. SCALE: 1-10 grain color scale (1= white, 2= cream, 3= light tan, 6= yellow, 10= black)" []
relationship: variable_of CO_350:0000071
relationship: variable_of CO_350:0005652
relationship: variable_of CO_350:0005414

[Term]
id: CO_350:0005054
name: Kernels per spikelet - kernels/spikelet
namespace: oat_trait
def: "TRAIT: Average number of kernels per spikelet METHOD: Calculation of the average number of kernels per spikelet, based on five typical spikelets. SCALE: kernels/spikelet" []
relationship: variable_of CO_350:0005653
relationship: variable_of CO_350:0005415
relationship: variable_of CO_350:0005910

[Term]
id: CO_350:0005055
name: Leaf biomass - 0-9 Rating
namespace: oat_trait
def: "TRAIT: An estimation of the leaf biomass METHOD: Estimation of the leaf biomass as a 'leafiness' rating on a 0-9 scale: very leafy= 3, few leaves=9. SCALE: 0-9 rating scale" []
relationship: variable_of CO_350:0005901
relationship: variable_of CO_350:0005654
relationship: variable_of CO_350:0005416

[Term]
id: CO_350:0005056
name: Panicle length - cm
namespace: oat_trait
def: "TRAIT: Average panicle length  METHOD: Calculation of the average panicle length from five mature panicles measured from the lowest panicle node to the tip of the apical spike SCALE: cm" []
relationship: variable_of CO_350:0000023
relationship: variable_of CO_350:0005655
relationship: variable_of CO_350:0005417

[Term]
id: CO_350:0005057
name: Spikelets per panicle - spikelets/panicle
namespace: oat_trait
def: "TRAIT: Average number of spikelets per panicle METHOD: Calculation of the average number of spikelets per panicle, based on five mature panicles SCALE: spikelets/panicle" []
relationship: variable_of CO_350:0005911
relationship: variable_of CO_350:0005418
relationship: variable_of CO_350:0005656

[Term]
id: CO_350:0005058
name: Avenanthramide content - 2c - ug/g
namespace: oat_trait
def: "TRAIT: Avenanthramide content METHOD: Direct measurement of the avenanthramide 2c content SCALE: ug/g" []
relationship: variable_of CO_350:0000035
relationship: variable_of CO_350:0000033
relationship: variable_of CO_350:0005657

[Term]
id: CO_350:0005059
name: Avenanthramide content - 2f - ug/g
namespace: oat_trait
def: "TRAIT: Avenanthramide content METHOD: Direct measurement of the avenanthramide 2f content SCALE: ug/g" []
relationship: variable_of CO_350:0005658
relationship: variable_of CO_350:0000033
relationship: variable_of CO_350:0000035

[Term]
id: CO_350:0005060
name: Avenanthramide content - 2p - ug/g
namespace: oat_trait
def: "TRAIT: Avenanthramide content METHOD: Direct measurement of the avenanthramide 2p content SCALE: ug/g" []
relationship: variable_of CO_350:0000035
relationship: variable_of CO_350:0000033
relationship: variable_of CO_350:0005659

[Term]
id: CO_350:0005061
name: Avenanthramide content - 5p - ug/g
namespace: oat_trait
def: "TRAIT: Avenanthramide content METHOD: Direct measurement of the avenanthramide 5p content SCALE: ug/g" []
relationship: variable_of CO_350:0000035
relationship: variable_of CO_350:0005660
relationship: variable_of CO_350:0000033

[Term]
id: CO_350:0005062
name: Avenanthramide relative abundance - A - relative abundance
namespace: oat_trait
def: "TRAIT: Relative abundance of avenanthramide estimated by UPLC METHOD: Estimation of the avenanthramide A relative abundance by UPLC SCALE: relative abundance" []
relationship: variable_of CO_350:0005661
relationship: variable_of CO_350:0005419
relationship: variable_of CO_350:0005912

[Term]
id: CO_350:0005063
name: Avenanthramide relative abundance - B - relative abundance
namespace: oat_trait
def: "TRAIT: Relative abundance of avenanthramide estimated by UPLC METHOD: Estimation of the avenanthramide B relative abundance by UPLC SCALE: relative abundance" []
relationship: variable_of CO_350:0005419
relationship: variable_of CO_350:0005662
relationship: variable_of CO_350:0005912

[Term]
id: CO_350:0005064
name: Avenanthramide relative abundance - C - relative abundance
namespace: oat_trait
def: "TRAIT: Relative abundance of avenanthramide estimated by UPLC METHOD: Estimation of the avenanthramide C relative abundance by UPLC SCALE: relative abundance" []
relationship: variable_of CO_350:0005419
relationship: variable_of CO_350:0005663
relationship: variable_of CO_350:0005912

[Term]
id: CO_350:0005065
name: Beta-glucan content - NIRS - percent
namespace: oat_trait
def: "TRAIT: Amount of beta-glucan present in the groat expressed as a percentage of the entire groat. METHOD: Measurement of beta-glucan content obtained using near-infrared spectroscopy (NIR). SCALE: percent" []
relationship: variable_of CO_350:0005664
relationship: variable_of CO_350:0000036
relationship: variable_of CO_350:0000011

[Term]
id: CO_350:0005066
name: Dehulling efficiency - %
namespace: oat_trait
def: "TRAIT: Efficiency of dehulling seed by a machine METHOD: Computation of the percentage of seed that is effectively dehulled by a Codema dehuller; calculated as the mass of seed before dehulling minus the amount of undehulled seed after processing, divided by the total mass before dehulling, and multiplied by 100 to give the percentage of seed that was successfully dehulled. SCALE: percent" []
relationship: variable_of CO_350:0005665
relationship: variable_of CO_350:0005420
relationship: variable_of CO_350:0000011

[Term]
id: CO_350:0005067
name: Dietary fiber content - HMW / Ethanol-insoluble - percent
namespace: oat_trait
def: "TRAIT: Dietary fiber content METHOD: Computation of the ethanol-insoluble high molecular weight dietary fiber content; measured on a dry weight basis using wet chemistry. SCALE: percent" []
relationship: variable_of CO_350:0005666
relationship: variable_of CO_350:0000042
relationship: variable_of CO_350:0000011

[Term]
id: CO_350:0005068
name: Dietary fiber content - HMW / Ethanol-soluble - percent
namespace: oat_trait
def: "TRAIT: Dietary fiber content METHOD: Computation of the ethanol-soluble high molecular weight dietary fiber content; measured on a dry weight basis using wet chemistry. SCALE: percent" []
relationship: variable_of CO_350:0000042
relationship: variable_of CO_350:0005667
relationship: variable_of CO_350:0000011

[Term]
id: CO_350:0005069
name: Dietary fiber content - HMW - percent
namespace: oat_trait
def: "TRAIT: Dietary fiber content METHOD: Computation of the high molecular weight dietary fiber content; measured on a dry weight basis using wet chemistry. SCALE: percent" []
relationship: variable_of CO_350:0000042
relationship: variable_of CO_350:0005668
relationship: variable_of CO_350:0000011

[Term]
id: CO_350:0005070
name: Dietary fiber content - LMW - percent
namespace: oat_trait
def: "TRAIT: Dietary fiber content METHOD: Computation of the low molecular weight dietary fiber content; measured on a dry weight basis using wet chemistry. SCALE: percent" []
relationship: variable_of CO_350:0000011
relationship: variable_of CO_350:0005669
relationship: variable_of CO_350:0000042

[Term]
id: CO_350:0005071
name: 3-acetyl-deoxynivalenol concentration - ppm
namespace: oat_trait
def: "TRAIT: Amount of the mycotoxin 3-acetyl-deoxynivalenol found in the grain after an infection by Fusarium sp. METHOD: Computation of the 3-acetyl-deoxynivalenol content SCALE: ppm" []
relationship: variable_of CO_350:0005670
relationship: variable_of CO_350:0005421
relationship: variable_of CO_350:0000047

[Term]
id: CO_350:0005072
name: Fatty acid content - C14:0 - %
namespace: oat_trait
def: "TRAIT: Fatty acid content of the grain METHOD: Measurement of fatty acid C14:0 content SCALE: percent" []
relationship: variable_of CO_350:0000011
relationship: variable_of CO_350:0005671
relationship: variable_of CO_350:0005422

[Term]
id: CO_350:0005073
name: Fatty acid content - C16:0 - %
namespace: oat_trait
def: "TRAIT: Fatty acid content of the grain METHOD: Measurement of fatty acid C16:0 content SCALE: percent" []
relationship: variable_of CO_350:0000011
relationship: variable_of CO_350:0005422
relationship: variable_of CO_350:0005672

[Term]
id: CO_350:0005074
name: Fatty acid content - C16:1 - %
namespace: oat_trait
def: "TRAIT: Fatty acid content of the grain METHOD: Measurement of fatty acid C16:1 content SCALE: percent" []
relationship: variable_of CO_350:0005673
relationship: variable_of CO_350:0005422
relationship: variable_of CO_350:0000011

[Term]
id: CO_350:0005075
name: Fatty acid content - C18:0 - %
namespace: oat_trait
def: "TRAIT: Fatty acid content of the grain METHOD: Measurement of fatty acid C18:0 content SCALE: percent" []
relationship: variable_of CO_350:0005422
relationship: variable_of CO_350:0005674
relationship: variable_of CO_350:0000011

[Term]
id: CO_350:0005076
name: Fatty acid content - C18:1(9) - %
namespace: oat_trait
def: "TRAIT: Fatty acid content of the grain METHOD: Measurement of fatty acid C18:1(9) content SCALE: percent" []
relationship: variable_of CO_350:0000011
relationship: variable_of CO_350:0005675
relationship: variable_of CO_350:0005422

[Term]
id: CO_350:0005077
name: Fatty acid content - C18:1* - %
namespace: oat_trait
def: "TRAIT: Fatty acid content of the grain METHOD: Measurement of fatty acid C18:1* content SCALE: percent" []
relationship: variable_of CO_350:0000011
relationship: variable_of CO_350:0005422
relationship: variable_of CO_350:0005676

[Term]
id: CO_350:0005078
name: Fatty acid content - C18:2 - %
namespace: oat_trait
def: "TRAIT: Fatty acid content of the grain METHOD: Measurement of fatty acid C18:2 content SCALE: percent" []
relationship: variable_of CO_350:0005677
relationship: variable_of CO_350:0005422
relationship: variable_of CO_350:0000011

[Term]
id: CO_350:0005079
name: Fatty acid content - C18:3 - %
namespace: oat_trait
def: "TRAIT: Fatty acid content of the grain METHOD: Measurement of fatty acid C18:3 content SCALE: percent" []
relationship: variable_of CO_350:0005678
relationship: variable_of CO_350:0005422
relationship: variable_of CO_350:0000011

[Term]
id: CO_350:0005080
name: Fatty acid content - C19:0 - %
namespace: oat_trait
def: "TRAIT: Fatty acid content of the grain METHOD: Measurement of fatty acid C19:0 content SCALE: percent" []
relationship: variable_of CO_350:0005679
relationship: variable_of CO_350:0005422
relationship: variable_of CO_350:0000011

[Term]
id: CO_350:0005081
name: Fatty acid content - C20:0 - %
namespace: oat_trait
def: "TRAIT: Fatty acid content of the grain METHOD: Measurement of fatty acid C20:0 content SCALE: percent" []
relationship: variable_of CO_350:0000011
relationship: variable_of CO_350:0005680
relationship: variable_of CO_350:0005422

[Term]
id: CO_350:0005082
name: Fatty acid content - C20:1 - %
namespace: oat_trait
def: "TRAIT: Fatty acid content of the grain METHOD: Measurement of fatty acid C20:1 content SCALE: percent" []
relationship: variable_of CO_350:0000011
relationship: variable_of CO_350:0005681
relationship: variable_of CO_350:0005422

[Term]
id: CO_350:0005083
name: Groat flour falling number - seconds
namespace: oat_trait
def: "TRAIT: Flour falling number is used as an indirect measurement of the alpha amylase content of the groat METHOD: Measurement of the amount of time it takes for a viscometer stirrer to fall a set distance through an aqueous gel created using groat flour. This indirectly measures the alpha amylase content of the groat, which becomes more abundant in grains that have suffered pre-harvest sprouting. An increase in alpha amylase in groat flour, along with other hydrolytic enzymes that are associated with pre-harvest sprouting, reduces the quality of the flour. SCALE: seconds" []
relationship: variable_of CO_350:0005682
relationship: variable_of CO_350:0005423
relationship: variable_of CO_350:0005913

[Term]
id: CO_350:0005084
name: Lutein content - %
namespace: oat_trait
def: "TRAIT: Lutein content METHOD: Measurement of the lutein content SCALE: percent" []
relationship: variable_of CO_350:0000011
relationship: variable_of CO_350:0005424
relationship: variable_of CO_350:0005683

[Term]
id: CO_350:0005085
name: Phytoene content - %
namespace: oat_trait
def: "TRAIT: Phytoene content METHOD: Measurement of the phytoene content SCALE: percent" []
relationship: variable_of CO_350:0005425
relationship: variable_of CO_350:0005684
relationship: variable_of CO_350:0000011

[Term]
id: CO_350:0005086
name: Phytofluene content - %
namespace: oat_trait
def: "TRAIT: Phytofluene content METHOD: Measurement of the phytofluene content SCALE: percent" []
relationship: variable_of CO_350:0000011
relationship: variable_of CO_350:0005685
relationship: variable_of CO_350:0005426

[Term]
id: CO_350:0005087
name: Seed quality - 1-7 seed quality scale
namespace: oat_trait
def: "TRAIT: Seed quality METHOD: Estimation of the seed qulaity on a 1-7 scale: 1= excellent, 7= poor SCALE: 1-7 seed quality scale (1= excellent, 7= poor)" []
relationship: variable_of CO_350:0005427
relationship: variable_of CO_350:0005686
relationship: variable_of CO_350:0005914

[Term]
id: CO_350:0005088
name: Silage moisture content - %
namespace: oat_trait
def: "TRAIT: Moisture content of silage. METHOD: Measurement of the moisture content of silage. SCALE: percent" []
relationship: variable_of CO_350:0005428
relationship: variable_of CO_350:0005687
relationship: variable_of CO_350:0000011

[Term]
id: CO_350:0005089
name: Total -tocopherol and -tocotrienol content - ug/g
namespace: oat_trait
def: "TRAIT: Measure of the total -tocopherol and -tocotrienol content METHOD: Measurement of the total -tocopherol and -tocotrienol content SCALE: ug/g" []
relationship: variable_of CO_350:0005688
relationship: variable_of CO_350:0005429
relationship: variable_of CO_350:0000035

[Term]
id: CO_350:0005090
name: Alpha-tocopherol content - ug/g
namespace: oat_trait
def: "TRAIT: Tocopherol concentration METHOD: Measurement of the alpha-tocopherol content SCALE: ug/g" []
relationship: variable_of CO_350:0000035
relationship: variable_of CO_350:0005689
relationship: variable_of CO_350:0000060

[Term]
id: CO_350:0005091
name: Beta-tocopherol content - ug/g
namespace: oat_trait
def: "TRAIT: Tocopherol concentration METHOD: Measurement of the beta-tocopherol content SCALE: ug/g" []
relationship: variable_of CO_350:0000035
relationship: variable_of CO_350:0000060
relationship: variable_of CO_350:0005690

[Term]
id: CO_350:0005092
name: Delta-tocopherol content - ug/g
namespace: oat_trait
def: "TRAIT: Tocopherol concentration METHOD: Measurement of the delta-tocopherol content SCALE: ug/g" []
relationship: variable_of CO_350:0000035
relationship: variable_of CO_350:0000060
relationship: variable_of CO_350:0005691

[Term]
id: CO_350:0005093
name: Gamma-tocopherol content - ug/g
namespace: oat_trait
def: "TRAIT: Tocopherol concentration METHOD: Measurement of the gamma-tocopherol content SCALE: ug/g" []
relationship: variable_of CO_350:0000035
relationship: variable_of CO_350:0000060
relationship: variable_of CO_350:0005692

[Term]
id: CO_350:0005094
name: Alpha-tocotrienol content - ug/g
namespace: oat_trait
def: "TRAIT: Tocotrienol concentration METHOD: Measurement of the alpha-tocotrienol content SCALE: ug/g" []
relationship: variable_of CO_350:0000035
relationship: variable_of CO_350:0000057
relationship: variable_of CO_350:0005693

[Term]
id: CO_350:0005095
name: Beta-tocotrienol content - ug/g
namespace: oat_trait
def: "TRAIT: Tocotrienol concentration METHOD: Measurement of the beta-tocotrienol content SCALE: ug/g" []
relationship: variable_of CO_350:0005694
relationship: variable_of CO_350:0000057
relationship: variable_of CO_350:0000035

[Term]
id: CO_350:0005096
name: Delta-tocotrienol content - ug/g
namespace: oat_trait
def: "TRAIT: Tocotrienol concentration METHOD: Measurement of the delta-tocotrienol content SCALE: ug/g" []
relationship: variable_of CO_350:0000035
relationship: variable_of CO_350:0000057
relationship: variable_of CO_350:0005695

[Term]
id: CO_350:0005097
name: Gamma-tocotrienol content - ug/g
namespace: oat_trait
def: "TRAIT: Tocotrienol concentration METHOD: Measurement of the gamma-tocotrienol content SCALE: ug/g" []
relationship: variable_of CO_350:0000035
relationship: variable_of CO_350:0000057
relationship: variable_of CO_350:0005696

[Term]
id: CO_350:0005098
name: Tunaxanthin content - %
namespace: oat_trait
def: "TRAIT: Tunaxanthin content METHOD: Measurement of the tunaxanthin content SCALE: percent" []
relationship: variable_of CO_350:0005697
relationship: variable_of CO_350:0005430
relationship: variable_of CO_350:0000011

[Term]
id: CO_350:0005099
name: Violaxanthin content - %
namespace: oat_trait
def: "TRAIT: Violaxanthin content METHOD: Measurement of the Violaxanthin content SCALE: percent" []
relationship: variable_of CO_350:0000011
relationship: variable_of CO_350:0005698
relationship: variable_of CO_350:0005431

[Term]
id: CO_350:0005100
name: Zeaxanthin content - %
namespace: oat_trait
def: "TRAIT: Zeaxanthin content METHOD: Measurement of the Zeaxanthin content SCALE: percent" []
relationship: variable_of CO_350:0000011
relationship: variable_of CO_350:0005699
relationship: variable_of CO_350:0005432
